update

semantics/compSpecFolScript.sml
@@ -1,35 +1,43 @@
-open HolKernel boolLib Parse bossLib pred_setTheory listTheory sumTheory combinTheory stringTheory ottTheory folStringTheory compSpecTheory compSpecMetaTheory;
+open HolKernel boolLib Parse bossLib;
+open pred_setTheory listTheory sumTheory combinTheory stringTheory;
+open ottTheory folStringTheory compSpecTheory compSpecUtilityTheory compSpecMetaTheory;
 
 val _ = new_theory "compSpecFol";
 
 Definition spec_interp_func:
- spec_interp_func (Mc : string -> 'a set) (MS : string -> ('a set) set) s l =
+ spec_interp_func (omega : 'a set)
+  (Mc : string -> 'a set)
+  (MS : string -> ('a set) set) s l =
   if      s = "c_comp" then INL (OUTL (EL 0 l) INTER OUTL (EL 1 l))
   else if s = "S_conj" then INR (OUTR (EL 0 l) INTER OUTR (EL 1 l))
-  else if s = "S_assume" then INR { b | !b'. b' IN OUTR (EL 0 l) ==> b INTER b' IN OUTR (EL 1 l) }
+  else if s = "S_assume" then
+   INR { B | B IN POW omega /\
+    !B'. B' IN OUTR (EL 0 l) ==> B INTER B' IN OUTR (EL 1 l) }
   else if s = "S_par" then INR (double_intersection (OUTR (EL 0 l)) (OUTR (EL 1 l)))
-  else if s = "S_compat" then INR { B | B <> {} }
-  else if s = "S_top" then INR { UNIV }
+  else if s = "S_compat" then INR { B | B IN POW omega  /\ B <> {} }
+  else if s = "S_top" then INR { omega }
   else if TAKE 8 s = "c_const_" then INL (Mc (DROP 8 s))
   else if TAKE 8 s = "S_const_" then INR (MS (DROP 8 s))
   else @x.T
 End
 
 Definition spec_interp_pred:
- spec_interp_pred s l =
+ spec_interp_pred omega s l =
   if      s = "P_implements" then OUTL (EL 0 l) IN OUTR (EL 1 l)
   else if s = "P_refines" then OUTR (EL 0 l) SUBSET OUTR (EL 1 l)
   else if s = "P_asserts" then downward_closed (OUTR (EL 0 l))
   else if s = "P_eq_c" then OUTL (EL 0 l) = OUTL (EL 1 l)
   else if s = "P_eq_S" then OUTR (EL 0 l) = OUTR (EL 1 l)
-  else if s = "P_is_c" then ISL (EL 0 l)
-  else if s = "P_is_S" then ISR (EL 0 l)
+  else if s = "P_is_c" then ISL (EL 0 l) /\ OUTL (EL 0 l) SUBSET omega
+  else if s = "P_is_S" then ISR (EL 0 l) /\ OUTR (EL 0 l) SUBSET POW omega
   else @x.T
 End
 
 Definition spec_interp_smodel:
- spec_interp_smodel Mc MS =
-  <| SDom := UNIV; SFun := spec_interp_func Mc MS; SPred := spec_interp_pred |>
+ spec_interp_smodel omega Mc MS =
+  <| SDom := \x. (ISL x /\ OUTL x SUBSET omega) \/ (ISR x /\ OUTR x SUBSET POW omega);
+     SFun := spec_interp_func omega Mc MS;
+     SPred := spec_interp_pred omega |>
 End
 
 Definition c2sterm:
@@ -41,7 +49,7 @@ Definition c2sterm:
 End
 
 Definition S2sterm:
- (S2sterm (S_const s) = SFn (STRCAT "S_const_" s) [])
+ (S2sterm (S_const (Sc_const s)) = SFn (STRCAT "S_const_" s) [])
  /\
  (S2sterm (S_conj S1 S2) = SFn "S_conj" [S2sterm S1; S2sterm S2])
  /\
@@ -51,9 +59,9 @@ Definition S2sterm:
  /\
  (S2sterm (S_var s) = SV (STRCAT "S_var_" s))
  /\
- (S2sterm S_compat = SFn "S_compat" [])
+ (S2sterm (S_const Sc_compat) = SFn "S_compat" [])
  /\
- (S2sterm S_top = SFn "S_top" [])
+ (S2sterm (S_const Sc_top) = SFn "S_top" [])
 End
 
 Definition P2sform:
@@ -79,6 +87,10 @@ Definition P2sform:
  /\
  (P2sform (P_and P1 P2) = SAnd (P2sform P1) (P2sform P2))
  /\
+ (P2sform (P_or P1 P2) = SOr (P2sform P1) (P2sform P2))
+ /\
+ (P2sform (P_not P) = SNot (P2sform P))
+ /\
  (P2sform (P_c_eq c1 c2) = SPred "P_eq_c" [c2sterm c1; c2sterm c2])
  /\
  (P2sform (P_S_eq S1 S2) = SPred "P_eq_S" [S2sterm S1; S2sterm S2])
@@ -92,19 +104,20 @@ Definition cSval:
 End
 
 Theorem c_sem_stermval:
- !Mc MS Mq MV c.
-  c_sem Mc Mq c = OUTL (stermval (spec_interp_smodel Mc MS) (cSval Mq MV) (c2sterm c))
+ !omega Mc MS Mq MV c.
+  c_sem Mc Mq c = OUTL (stermval (spec_interp_smodel omega Mc MS) (cSval Mq MV) (c2sterm c))
 Proof
- strip_tac >> strip_tac >> strip_tac >> strip_tac >> 
+ strip_tac >> strip_tac >> strip_tac >> strip_tac >> strip_tac >> 
  Induct_on `c` >> rw [c_sem,stermval,spec_interp_smodel,c2sterm,spec_interp_func,cSval]
 QED
 
 Theorem S_sem_stermval:
- !Mc MS Mq MV S.
-  S_sem MS MV S = OUTR (stermval (spec_interp_smodel Mc MS) (cSval Mq MV) (S2sterm S))
+ !omega Mc MS Mq MV S.
+  S_sem omega MS MV S = OUTR (stermval (spec_interp_smodel omega Mc MS) (cSval Mq MV) (S2sterm S))
 Proof
- strip_tac >> strip_tac >> strip_tac >> strip_tac >> strip_tac >>
- Induct_on `S'` >> rw [S_sem,stermval,spec_interp_smodel,S2sterm,spec_interp_func,cSval]
+ strip_tac >> strip_tac >> strip_tac >> strip_tac >> strip_tac >> strip_tac >>
+ Induct_on `S'` >> rw [S_sem,stermval,spec_interp_smodel,S2sterm,spec_interp_func,cSval] >>
+ Cases_on `S'` >> rw [S_sem,stermval,spec_interp_smodel,S2sterm,spec_interp_func,cSval]
 QED
 
 Theorem ISL_OUTL_eq:
@@ -146,9 +159,23 @@ Proof
  ]
 QED
 
+Theorem APPLY_UPDATE_SUBSET:
+ !M omega s0 x.
+  (!s. M s SUBSET omega) /\
+  x SUBSET omega ==>
+  !s. ((s0 =+ x) M) s SUBSET omega
+Proof
+ rw [APPLY_UPDATE_THM] >>
+ Cases_on `s0 = s` >> rw []
+QED
+
 Theorem P_sem_sholds:
- !Mc MS Mq MV P.
-  P_sem Mc MS Mq MV P <=> sholds (spec_interp_smodel Mc MS) (cSval Mq MV) (P2sform P)
+ !omega Mc MS Mq MV P.
+  (!s. Mc s SUBSET omega) /\
+  (!s. Mq s SUBSET omega) /\
+  (!s. MS s SUBSET POW omega) /\
+  (!s. MV s SUBSET POW omega) ==>
+  (P_sem omega Mc MS Mq MV P <=> sholds (spec_interp_smodel omega Mc MS) (cSval Mq MV) (P2sform P))
 Proof
  Induct_on `P` >> rw [P_sem,sholds,P2sform,spec_interp_smodel,spec_interp_pred] >| [
   METIS_TAC [c_sem_stermval,S_sem_stermval,spec_interp_smodel],
@@ -160,51 +187,88 @@ Proof
   Q.ABBREV_TAC `cvars = STRING #"c" (STRING #"_" (STRING #"v" 
    (STRING #"a" (STRING #"r" (STRING #"_" s)))))` >>
   rw [APPLY_UPDATE_THM] >>
-  EQ_TAC >> rw [] >-
-   (Cases_on `a` >> fs [] >>
-    `sholds (spec_interp_smodel Mc MS) (cSval ((s =+ x) Mq) MV) (P2sform P)`    
-     by fs [spec_interp_smodel] >>
-    METIS_TAC [spec_interp_smodel,cSval_UPDATE_Mq,Abbr `cvars`,STRCAT_def]) >>
-  `sholds (spec_interp_smodel Mc MS) ((cvars =+ INL qs) (cSval Mq MV)) (P2sform P)`    
-   by fs [spec_interp_smodel,INL] >>
-  METIS_TAC [spec_interp_smodel,cSval_UPDATE_Mq,Abbr `cvars`,STRCAT_def],
+  EQ_TAC >> rw [] >| [
+   Cases_on `a` >> fs [] >>
+   `!s'. (s =+ x) Mq s' SUBSET omega` by METIS_TAC [APPLY_UPDATE_SUBSET] >>
+   `sholds (spec_interp_smodel omega Mc MS) (cSval ((s =+ x) Mq) MV) (P2sform P)`    
+    by METIS_TAC [spec_interp_smodel] >>
+   METIS_TAC [spec_interp_smodel,cSval_UPDATE_Mq,Abbr `cvars`,STRCAT_def],
+
+   METIS_TAC [NOT_ISL_ISR],
+
+   `!s'. (s =+ qs) Mq s' SUBSET omega` by METIS_TAC [APPLY_UPDATE_SUBSET] >>
+   `sholds (spec_interp_smodel omega Mc MS) ((cvars =+ INL qs) (cSval Mq MV)) (P2sform P)`    
+    by fs [spec_interp_smodel,INL] >>
+   METIS_TAC [spec_interp_smodel,cSval_UPDATE_Mq,Abbr `cvars`,STRCAT_def]
+  ],
 
   Q.ABBREV_TAC `cvars = STRING #"c" (STRING #"_" (STRING #"v" 
    (STRING #"a" (STRING #"r" (STRING #"_" s)))))` >>
   rw [APPLY_UPDATE_THM] >>
-  EQ_TAC >> rw [] >-
-   (Q.EXISTS_TAC `INL qs` >> rw [] >>
-    METIS_TAC [spec_interp_smodel,cSval_UPDATE_Mq,Abbr `cvars`,STRCAT_def]) >>
-  Cases_on `a` >> fs [] >>
-  Q.EXISTS_TAC `x` >> rw [] >>
-  METIS_TAC [spec_interp_smodel,cSval_UPDATE_Mq,Abbr `cvars`,STRCAT_def],
+  EQ_TAC >> rw [] >| [
+   Q.EXISTS_TAC `INL qs` >> rw [] >>
+   `!s'. (s =+ qs) Mq s' SUBSET omega` by METIS_TAC [APPLY_UPDATE_SUBSET] >>
+   METIS_TAC [spec_interp_smodel,cSval_UPDATE_Mq,Abbr `cvars`,STRCAT_def],
+
+   Cases_on `a` >> fs [] >>
+   Q.EXISTS_TAC `x` >> rw [] >>
+   `!s'. (s =+ x) Mq s' SUBSET omega` by METIS_TAC [APPLY_UPDATE_SUBSET] >>
+   METIS_TAC [spec_interp_smodel,cSval_UPDATE_Mq,Abbr `cvars`,STRCAT_def],
+
+   METIS_TAC [NOT_ISL_ISR]
+  ],
 
   Q.ABBREV_TAC `Svars = STRING #"S" (STRING #"_" (STRING #"v" 
    (STRING #"a" (STRING #"r" (STRING #"_" s)))))` >>
   rw [APPLY_UPDATE_THM] >>
-  EQ_TAC >> rw [] >-
-   (Cases_on `a` >> fs [] >>
-    `sholds (spec_interp_smodel Mc MS) (cSval Mq ((s =+ y) MV)) (P2sform P)`    
-     by fs [spec_interp_smodel] >>
-    METIS_TAC [spec_interp_smodel,cSval_UPDATE_MV,Abbr `Svars`,STRCAT_def]) >>
-  `sholds (spec_interp_smodel Mc MS) ((Svars =+ INR Vs) (cSval Mq MV)) (P2sform P)`    
-   by fs [spec_interp_smodel,INR] >>
-  METIS_TAC [spec_interp_smodel,cSval_UPDATE_MV,Abbr `Svars`,STRCAT_def],
+  EQ_TAC >> rw [] >| [
+   METIS_TAC [NOT_ISL_ISR],
+
+   Cases_on `a` >> fs [] >>
+   `!s'. (s =+ y) MV s' SUBSET POW omega` by METIS_TAC [APPLY_UPDATE_SUBSET] >>
+   `sholds (spec_interp_smodel omega Mc MS) (cSval Mq ((s =+ y) MV)) (P2sform P)`    
+    by METIS_TAC [spec_interp_smodel] >>
+   METIS_TAC [spec_interp_smodel,cSval_UPDATE_MV,Abbr `Svars`,STRCAT_def],
+
+   `!s'. (s =+ Vs) MV s' SUBSET POW omega` by METIS_TAC [APPLY_UPDATE_SUBSET] >>
+   `sholds (spec_interp_smodel omega Mc MS) ((Svars =+ INR Vs) (cSval Mq MV)) (P2sform P)`    
+    by fs [spec_interp_smodel,INR] >>
+   METIS_TAC [spec_interp_smodel,cSval_UPDATE_MV,Abbr `Svars`,STRCAT_def]
+  ],
 
   Q.ABBREV_TAC `Svars = STRING #"S" (STRING #"_" (STRING #"v" 
    (STRING #"a" (STRING #"r" (STRING #"_" s)))))` >>
   rw [APPLY_UPDATE_THM] >>
-  EQ_TAC >> rw [] >-
-   (Q.EXISTS_TAC `INR Vs` >> rw [] >>
-    METIS_TAC [spec_interp_smodel,cSval_UPDATE_MV,Abbr `Svars`,STRCAT_def]) >>
-  Cases_on `a` >> fs [] >>
-  Q.EXISTS_TAC `y` >> rw [] >>
-  METIS_TAC [spec_interp_smodel,cSval_UPDATE_MV,Abbr `Svars`,STRCAT_def],
+  EQ_TAC >> rw [] >| [
+   Q.EXISTS_TAC `INR Vs` >> rw [] >>
+   `!s'. (s =+ Vs) MV s' SUBSET POW omega` by METIS_TAC [APPLY_UPDATE_SUBSET] >>
+   METIS_TAC [spec_interp_smodel,cSval_UPDATE_MV,Abbr `Svars`,STRCAT_def],
+
+   METIS_TAC [NOT_ISL_ISR],
+   
+   Cases_on `a` >> fs [] >>   
+   Q.EXISTS_TAC `y` >> rw [] >>
+   `!s'. (s =+ y) MV s' SUBSET POW omega` by METIS_TAC [APPLY_UPDATE_SUBSET] >>
+   METIS_TAC [spec_interp_smodel,cSval_UPDATE_MV,Abbr `Svars`,STRCAT_def]
+  ],
 
   METIS_TAC [c_sem_stermval,S_sem_stermval,spec_interp_smodel],
 
   METIS_TAC [S_sem_stermval,S_sem_stermval,spec_interp_smodel]
  ]
+QED
+
+Theorem P_sem_holds:
+ !omega Mc MS Mq MV P.
+  (!s. Mc s SUBSET omega) /\
+  (!s. Mq s SUBSET omega) /\
+  (!s. MS s SUBSET POW omega) /\
+  (!s. MV s SUBSET POW omega) ==>
+  (P_sem omega Mc MS Mq MV P <=>
+   holds (smodel2model (spec_interp_smodel omega Mc MS)) ((cSval Mq MV) o n2s) (sform2form (P2sform P)))
+Proof
+ once_rewrite_tac [GSYM sholds_holds] >>
+ rw [P_sem_sholds]
 QED
 
 val _ = export_theory ();
