semantics/compSpecMetaScript.sml
@@ -1,4 +1,7 @@
-open HolKernel boolLib Parse bossLib pred_setTheory listTheory combinTheory ottTheory compSpecUtilityTheory compSpecTheory;
+open HolKernel boolLib Parse bossLib;
+open pred_setTheory listTheory combinTheory;
+open stringTheory string_numTheory;
+open ottTheory compSpecUtilityTheory compSpecTheory;
 
 (* ====================================== *)
 (* Compositional specification metatheory *)
@@ -10,15 +13,13 @@ val _ = new_theory "compSpecMeta";
 (* Auxiliary definitions *)
 (* --------------------- *)
 
-Definition list_S_par:
- (list_S_par S [] = S)
- /\
- (list_S_par S (S'::Sl) = S_par S (list_S_par S' Sl))
+Definition S_par_list:
+ S_par_list (S::Sl) = FOLDL (\S0. S_par S0) S Sl
 End
 
-Definition list_S_par_alt:
- list_S_par_alt (S:S) Sl = FOLDL (\S'. S_par S') S Sl
-End
+(*
+EVAL ``S_par_list (S_const Sc_top::S_const Sc_compat::S_const (Sc_const "test")::[])``
+*)
 
 (* -------------------- *)
 (* Semantic definitions *)
@@ -33,74 +34,116 @@ Definition c_sem:
 End
 
 Definition S_sem:
- (S_sem MS MV (S_const sn) = MS sn)
+ (S_sem omega MS MV (S_const (Sc_const sn)) = MS sn)
  /\
- (S_sem MS MV (S_conj S1 S2) = S_sem MS MV S1 INTER S_sem MS MV S2)
+ (S_sem omega MS MV (S_conj S1 S2) = S_sem omega MS MV S1 INTER S_sem omega MS MV S2)
  /\
- (S_sem MS MV (S_assume S1 S2) =
-  { b | !b'. b' IN S_sem MS MV S1 ==> b INTER b' IN S_sem MS MV S2 })
+ (S_sem omega MS MV (S_assume S1 S2) =
+  { B | B IN POW omega /\
+    !B'. B' IN S_sem omega MS MV S1 ==> B INTER B' IN S_sem omega MS MV S2 })
  /\
- (S_sem MS MV (S_par S1 S2) =
-  double_intersection (S_sem MS MV S1) (S_sem MS MV S2))
+ (S_sem omega MS MV (S_par S1 S2) =
+  double_intersection (S_sem omega MS MV S1) (S_sem omega MS MV S2))
  /\
- (S_sem MS MV (S_var V) = MV V)
+ (S_sem omega MS MV (S_var V) = MV V)
  /\
- (S_sem MS MV S_compat = { B | B <> {} })
+ (S_sem omega MS MV (S_const Sc_compat) = { B | B IN POW omega /\ B <> {} })
  /\
- (S_sem MS MV S_top = { UNIV })
+ (S_sem omega MS MV (S_const Sc_top) = { omega })
 End
 
 Definition P_sem:
- (P_sem Mc MS Mq MV (P_implements c S) =
-  (c_sem Mc Mq c IN S_sem MS MV S))
+ (P_sem omega Mc MS Mq MV (P_implements c S) =
+  (c_sem Mc Mq c IN S_sem omega MS MV S))
  /\
- (P_sem Mc MS Mq MV (P_refines S1 S2) =
-  (S_sem MS MV S1 SUBSET S_sem MS MV S2))
+ (P_sem omega Mc MS Mq MV (P_refines S1 S2) =
+  (S_sem omega MS MV S1 SUBSET S_sem omega MS MV S2))
  /\
- (P_sem Mc MS Mq MV (P_asserts S) =
-  (downward_closed (S_sem MS MV S)))
+ (P_sem omega Mc MS Mq MV (P_asserts S) =
+  (downward_closed (S_sem omega MS MV S)))
  /\
- (P_sem Mc MS Mq MV (P_forall_c q P) =
-  (!qs. P_sem Mc MS ((q =+ qs) Mq) MV P))
+ (P_sem omega Mc MS Mq MV (P_forall_c q P) =
+  (!qs. qs SUBSET omega ==> P_sem omega Mc MS ((q =+ qs) Mq) MV P))
  /\
- (P_sem Mc MS Mq MV (P_exists_c q P) =
-  (?qs. P_sem Mc MS ((q =+ qs) Mq) MV P))
+ (P_sem omega Mc MS Mq MV (P_exists_c q P) =
+  (?qs. qs SUBSET omega /\ P_sem omega Mc MS ((q =+ qs) Mq) MV P))
  /\
- (P_sem Mc MS Mq MV (P_forall_S V P) =
-  (!Vs. P_sem Mc MS Mq ((V =+ Vs) MV) P))
+ (P_sem omega Mc MS Mq MV (P_forall_S V P) =
+  (!Vs. Vs SUBSET POW omega ==> P_sem omega Mc MS Mq ((V =+ Vs) MV) P))
  /\
- (P_sem Mc MS Mq MV (P_exists_S V P) =
-  (?Vs. P_sem Mc MS Mq ((V =+ Vs) MV) P))
+ (P_sem omega Mc MS Mq MV (P_exists_S V P) =
+  (?Vs. Vs SUBSET POW omega /\ P_sem omega Mc MS Mq ((V =+ Vs) MV) P))
  /\
- (P_sem Mc MS Mq MV (P_implies P1 P2) =
-  (P_sem Mc MS Mq MV P1 ==> P_sem Mc MS Mq MV P2))
+ (P_sem omega Mc MS Mq MV (P_implies P1 P2) =
+  (P_sem omega Mc MS Mq MV P1 ==> P_sem omega Mc MS Mq MV P2))
  /\
- (P_sem Mc MS Mq MV (P_and P1 P2) =
-  (P_sem Mc MS Mq MV P1 /\ P_sem Mc MS Mq MV P2))
+ (P_sem omega Mc MS Mq MV (P_and P1 P2) =
+  (P_sem omega Mc MS Mq MV P1 /\ P_sem omega Mc MS Mq MV P2))
  /\
- (P_sem Mc MS Mq MV (P_c_eq c1 c2) =
+ (P_sem omega Mc MS Mq MV (P_or P1 P2) =
+  (P_sem omega Mc MS Mq MV P1 \/ P_sem omega Mc MS Mq MV P2))
+ /\
+ (P_sem omega Mc MS Mq MV (P_not P) =
+  ~(P_sem omega Mc MS Mq MV P))
+ /\
+ (P_sem omega Mc MS Mq MV (P_c_eq c1 c2) =
   (c_sem Mc Mq c1 = c_sem Mc Mq c2))
  /\
- (P_sem Mc MS Mq MV (P_S_eq S1 S2) =
-  (S_sem MS MV S1 = S_sem MS MV S2))
+ (P_sem omega Mc MS Mq MV (P_S_eq S1 S2) =
+  (S_sem omega MS MV S1 = S_sem omega MS MV S2))
 End
 
 Definition spec_compositionality:
- spec_compositionality Mc MS Mq MV S0 Sl S =
-  (P_sem Mc MS Mq MV (P_refines (list_S_par S0 Sl) S))
+ spec_compositionality omega Mc MS Mq MV Sl S =
+  (P_sem omega Mc MS Mq MV (P_refines (S_par_list Sl) S))
 End
 
-(* FIXME: valuations not needed *)
 Definition spec_system_sound:
- spec_system_sound R Mc MS Mq MV =
-  !G P. (!P0. P0 IN G ==> P_sem Mc MS Mq MV P0) /\
+  spec_system_sound R omega =
+  (!Mc MS Mq MV G P.
+    (!s. Mc s SUBSET omega) /\
+    (!s. Mq s SUBSET omega) /\
+    (!s. MS s SUBSET POW omega) /\
+    (!s. MV s SUBSET POW omega) /\
+    (!P0. P0 IN G ==> P_sem omega Mc MS Mq MV P0) /\
     R G P ==>
-    P_sem Mc MS Mq MV P
+    P_sem omega Mc MS Mq MV P)
 End
 
 (* --------------- *)
 (* Utility results *)
 (* --------------- *)
+
+Theorem q_BIGUNION_IMAGE_fvP_c:
+ !q (G:G).
+  q IN BIGUNION (IMAGE fv_P_c G) <=> (?P. P IN G /\ q IN fv_P_c P)
+Proof
+ rw [BIGUNION] >>
+ METIS_TAC []
+QED
+
+Theorem FINITE_IMAGE_s2n:
+ !s. FINITE s ==> FINITE (IMAGE s2n s)
+Proof
+ rw [INJECTIVE_IMAGE_FINITE]
+QED
+
+Theorem SVARIANT_FINITE:
+ !s. FINITE s ==> SVARIANT s NOTIN s
+Proof
+ rw [SVARIANT_def] >>
+ `FINITE (IMAGE s2n s)` by METIS_TAC [FINITE_IMAGE_s2n] >>
+ `!x. x IN (IMAGE s2n s) ==> x <= MAX_SET (IMAGE s2n s)`
+  by METIS_TAC [in_max_set] >>
+ strip_tac >>
+ sg `MAX_SET (IMAGE s2n s) + 1 NOTIN (IMAGE s2n s)` >-
+  (strip_tac >>
+   `MAX_SET (IMAGE s2n s) + 1 <= MAX_SET (IMAGE s2n s)` by METIS_TAC [] >>
+   DECIDE_TAC) >>
+ `MAX_SET (IMAGE s2n s) + 1 IN (IMAGE s2n s)` suffices_by METIS_TAC [] >>
+ `s2n (n2s (MAX_SET (IMAGE s2n s) + 1)) IN IMAGE s2n s` by METIS_TAC [IMAGE_IN] >>
+ METIS_TAC [s2n_n2s] 
+QED
 
 Theorem fv_c_eq_c_sem:
  !Mc Mq Mq' c. (!q. q IN fv_c c ==> Mq q = Mq' q) ==>
@@ -111,38 +154,41 @@ Proof
 QED
 
 Theorem fv_S_eq_S_sem:
- !MS MV MV' S'. (!V. V IN fv_S S' ==> MV V = MV' V) ==>
-  S_sem MS MV S' = S_sem MS MV' S'
+ !omega MS MV MV' S'. (!V. V IN fv_S S' ==> MV V = MV' V) ==>
+  S_sem omega MS MV S' = S_sem omega MS MV' S'
 Proof
- strip_tac >> strip_tac >> strip_tac >>
- Induct_on `S'` >> rw [S_sem,fv_S]
+ strip_tac >> strip_tac >> strip_tac >> strip_tac >>
+ Induct_on `S'` >> rw [S_sem,fv_S] >>
+ Cases_on `S'` >> rw [S_sem]
 QED
 
 Theorem fv_P_c_eq_P_sem:
- !Mc MS P Mq Mq' MV. 
+ !omega Mc MS P Mq Mq' MV. 
   (!q. q IN fv_P_c P ==> Mq q = Mq' q) ==>
-  P_sem Mc MS Mq MV P = P_sem Mc MS Mq' MV P
+  P_sem omega Mc MS Mq MV P = P_sem omega Mc MS Mq' MV P
 Proof
- strip_tac >> strip_tac >>
+ strip_tac >> strip_tac >> strip_tac >>
  Induct_on `P` >> rw [P_sem,fv_P_c] >| [
   METIS_TAC [fv_c_eq_c_sem],
 
   EQ_TAC >> rw [] >>
   `!q. q IN fv_P_c P ==> ((s =+ qs) Mq) q = ((s =+ qs) Mq') q`
    by rw [APPLY_UPDATE_THM] >>
-  `P_sem Mc MS ((s =+ qs) Mq) MV P <=> P_sem Mc MS ((s =+ qs) Mq') MV P`
-   by (Q.PAT_X_ASSUM `!M1 M2 M3. Q ==> R` (STRIP_ASSUME_TAC o
-    (Q.SPECL [`(s =+ qs) Mq`,`(s =+ qs) Mq'`])) >>
+  sg `P_sem omega Mc MS ((s =+ qs) Mq) MV P <=> P_sem omega Mc MS ((s =+ qs) Mq') MV P` >-
+   (Q.PAT_X_ASSUM `!M1 M2 M3. Q ==> R`
+     (STRIP_ASSUME_TAC o (Q.SPECL [`(s =+ qs) Mq`,`(s =+ qs) Mq'`])) >>
     METIS_TAC []) >>
   METIS_TAC [],
 
   EQ_TAC >> rw [] >>
   `!q. q IN fv_P_c P ==> ((s =+ qs) Mq) q = ((s =+ qs) Mq') q`
    by rw [APPLY_UPDATE_THM] >>
-  `P_sem Mc MS ((s =+ qs) Mq) MV P <=> P_sem Mc MS ((s =+ qs) Mq') MV P`
+  `P_sem omega Mc MS ((s =+ qs) Mq) MV P <=> P_sem omega Mc MS ((s =+ qs) Mq') MV P`
    by (Q.PAT_X_ASSUM `!M1 M2 M3. Q ==> R` (STRIP_ASSUME_TAC o
     (Q.SPECL [`(s =+ qs) Mq`,`(s =+ qs) Mq'`])) >>
     METIS_TAC []) >>
+  METIS_TAC [],
+
   METIS_TAC [],
 
   METIS_TAC [],
@@ -158,11 +204,11 @@ Proof
 QED
 
 Theorem fv_P_S_eq_P_sem:
- !Mc MS P MV MV' Mq. 
+ !omega Mc MS P MV MV' Mq. 
   (!V. V IN fv_P_S P ==> MV V = MV' V) ==>
-  P_sem Mc MS Mq MV P = P_sem Mc MS Mq MV' P
+  P_sem omega Mc MS Mq MV P = P_sem omega Mc MS Mq MV' P
 Proof
- strip_tac >> strip_tac >>
+ strip_tac >> strip_tac >> strip_tac >>
  Induct_on `P` >> rw [P_sem,fv_P_S] >| [
   METIS_TAC [fv_S_eq_S_sem],
 
@@ -177,7 +223,7 @@ Proof
   EQ_TAC >> rw [] >>
   `!V. V IN fv_P_S P ==> ((s =+ Vs) MV) V = ((s =+ Vs) MV') V`
    by rw [APPLY_UPDATE_THM] >>
-  `P_sem Mc MS Mq ((s =+ Vs) MV) P <=> P_sem Mc MS Mq ((s =+ Vs) MV') P`
+  `P_sem omega Mc MS Mq ((s =+ Vs) MV) P <=> P_sem omega Mc MS Mq ((s =+ Vs) MV') P`
    by (Q.PAT_X_ASSUM `!M1 M2 M3. Q ==> R` (STRIP_ASSUME_TAC o
     (Q.SPECL [`(s =+ Vs) MV`,`(s =+ Vs) MV'`])) >>
     METIS_TAC []) >>
@@ -186,10 +232,12 @@ Proof
   EQ_TAC >> rw [] >>
   `!V. V IN fv_P_S P ==> ((s =+ Vs) MV) V = ((s =+ Vs) MV') V`
    by rw [APPLY_UPDATE_THM] >>
-  `P_sem Mc MS Mq ((s =+ Vs) MV) P <=> P_sem Mc MS Mq ((s =+ Vs) MV') P`
+  `P_sem omega Mc MS Mq ((s =+ Vs) MV) P <=> P_sem omega Mc MS Mq ((s =+ Vs) MV') P`
    by (Q.PAT_X_ASSUM `!M1 M2 M3. Q ==> R` (STRIP_ASSUME_TAC o
     (Q.SPECL [`(s =+ Vs) MV`,`(s =+ Vs) MV'`])) >>
     METIS_TAC []) >>
+  METIS_TAC [],
+
   METIS_TAC [],
 
   METIS_TAC [],
@@ -200,22 +248,85 @@ Proof
  ]
 QED
 
+Theorem fv_c_notin_c_sem:
+ !Mc Mq c q qs. q NOTIN fv_c c ==>
+  c_sem Mc Mq c = c_sem Mc ((q =+ qs) Mq) c
+Proof
+ rw [] >>
+ match_mp_tac fv_c_eq_c_sem >>
+ rw [] >>
+ `q <> q'` by METIS_TAC [] >>
+ rw [APPLY_UPDATE_THM]
+QED
+
 Theorem fv_c_empty_c_sem:
  !Mc Mq c q qs. fv_c c = {} ==>
   c_sem Mc Mq c = c_sem Mc ((q =+ qs) Mq) c
 Proof
  rw [] >> 
- match_mp_tac fv_c_eq_c_sem >>
- rw []
+ `q NOTIN fv_c c` by fs [] >>
+ METIS_TAC [fv_c_notin_c_sem]
 QED
 
-Theorem fv_S_empty_S_sem:
- !MS MV S V Vs. fv_S S = {} ==>
-  S_sem MS MV S = S_sem MS ((V =+ Vs) MV) S
+Theorem fv_P_c_notin_P_sem:
+ !omega Mc MS Mq MV P q qs. q NOTIN fv_P_c P ==>
+  (P_sem omega Mc MS Mq MV P <=> P_sem omega Mc MS ((q =+ qs) Mq) MV P)
+Proof
+ rw [] >>
+ match_mp_tac fv_P_c_eq_P_sem >>
+ rw [] >>
+ `q <> q'` by METIS_TAC [] >>
+ rw [APPLY_UPDATE_THM]
+QED
+
+Theorem fv_S_notin_S_sem:
+ !omega MS MV S V Vs. V NOTIN fv_S S ==>
+  S_sem omega MS MV S = S_sem omega MS ((V =+ Vs) MV) S
 Proof
  rw [] >>
  match_mp_tac fv_S_eq_S_sem >>
- rw []
+ rw [] >>
+ `V <> V'` by METIS_TAC [] >>
+ rw [APPLY_UPDATE_THM]
+QED
+
+Theorem fv_S_empty_S_sem:
+ !omega MS MV S V Vs. fv_S S = {} ==>
+  S_sem omega MS MV S = S_sem omega MS ((V =+ Vs) MV) S
+Proof
+ rw [] >> 
+ `V NOTIN fv_S S'` by fs [] >>
+ METIS_TAC [fv_S_notin_S_sem]
+QED
+
+Theorem c_sem_omega:
+ !omega Mc Mq.
+ (!s. Mc s SUBSET omega) /\
+ (!s. Mq s SUBSET omega) ==>
+ !c0. c_sem Mc Mq c0 SUBSET omega
+Proof
+ strip_tac >> strip_tac >> strip_tac >> strip_tac >>
+ Induct_on `c0` >> rw [c_sem] >>
+ fs [SUBSET_DEF,INTER_DEF]
+QED
+
+Theorem S_sem_omega:
+ !omega MS MV.
+ (!s. MS s SUBSET POW omega) /\
+ (!s. MV s SUBSET POW omega) ==>
+ !S0. S_sem omega MS MV S0 SUBSET POW omega
+Proof
+ strip_tac >> strip_tac >> strip_tac >> strip_tac >>
+ Induct_on `S0` >> rw [S_sem] >| [
+  Cases_on `S'` >> rw [S_sem] >-
+  rw [SUBSET_DEF,IN_POW] >>
+  rw [IN_POW],  
+  fs [SUBSET_DEF,INTER_DEF],
+  rw [SUBSET_DEF],
+  rw [double_intersection,SUBSET_DEF] >>
+  rw [INTER_DEF,IN_POW,SUBSET_DEF] >>
+  METIS_TAC [IN_POW,SUBSET_DEF]
+ ] 
 QED
 
 (* --------------------- *)
@@ -243,140 +354,161 @@ Proof
 QED
 
 Theorem S_sem_IN_assume_IN:
- !MS MV A1 G1 a.
-  a IN S_sem MS MV (S_assume A1 G1) /\
-  a IN S_sem MS MV A1 ==>
-  a IN S_sem MS MV G1
-Proof
- rw [S_sem] >> METIS_TAC [INTER_IDEMPOT]
-QED
-
-Theorem S_sem_IN_assume_IN:
- !MS MV A1 G1 a.
-  a IN S_sem MS MV (S_assume A1 G1) /\
-  a IN S_sem MS MV A1 ==>
-  a IN S_sem MS MV G1
+ !omega MS MV A1 G1 a.
+  a IN S_sem omega MS MV (S_assume A1 G1) /\
+  a IN S_sem omega MS MV A1 ==>
+  a IN S_sem omega MS MV G1
 Proof
  rw [S_sem] >> METIS_TAC [INTER_IDEMPOT]
 QED
 
 Theorem S_sem_IN_par_IN:
- !MS MV A1 G1 x.
-  x IN S_sem MS MV (S_par A1 G1) <=>
-  ?a b. x = a INTER b /\ a IN S_sem MS MV A1 /\ b IN S_sem MS MV G1
+ !omega MS MV A1 G1 x.
+  x IN S_sem omega MS MV (S_par A1 G1) <=>
+  ?a b. x = a INTER b /\ a IN S_sem omega MS MV A1 /\ b IN S_sem omega MS MV G1
 Proof
  rw [S_sem,double_intersection]
 QED
 
 Theorem S_sem_conj_IDEM:
- !MS MV S. S_sem MS MV (S_conj S S) = S_sem MS MV S
+ !omega MS MV S. S_sem omega MS MV (S_conj S S) = S_sem omega MS MV S
 Proof
  rw [S_sem,INTER_IDEMPOT]
 QED
 
 Theorem S_sem_conj_ASSOC:
- !MS MV S1 S2 S3.
-  S_sem MS MV (S_conj S1 (S_conj S2 S3)) = S_sem MS MV (S_conj (S_conj S1 S2) S3)
+ !omega MS MV S1 S2 S3.
+  S_sem omega MS MV (S_conj S1 (S_conj S2 S3)) = S_sem omega MS MV (S_conj (S_conj S1 S2) S3)
 Proof
  rw [S_sem,INTER_ASSOC]
 QED
 
 Theorem S_sem_conj_COMM:
- !MS MV S1 S2.
-  S_sem MS MV (S_conj S1 S2) = S_sem MS MV (S_conj S2 S1)
+ !omega MS MV S1 S2.
+  S_sem omega MS MV (S_conj S1 S2) = S_sem omega MS MV (S_conj S2 S1)
 Proof
  rw [S_sem,INTER_COMM]
 QED
 
 Theorem S_sem_par_ASSOC:
- !MS MV S1 S2 S3.
-  S_sem MS MV (S_par S1 (S_par S2 S3)) = S_sem MS MV (S_par (S_par S1 S2) S3)
+ !omega MS MV S1 S2 S3.
+  S_sem omega MS MV (S_par S1 (S_par S2 S3)) = S_sem omega MS MV (S_par (S_par S1 S2) S3)
 Proof
  rw [S_sem,double_intersection_ASSOC]
 QED
 
 Theorem S_sem_par_COMM:
- !MS MV S1 S2. S_sem MS MV (S_par S1 S2) = S_sem MS MV (S_par S2 S1)
+ !omega MS MV S1 S2.
+  S_sem omega MS MV (S_par S1 S2) = S_sem omega MS MV (S_par S2 S1)
 Proof
  rw [S_sem,double_intersection_COMM]
 QED
 
 Theorem proposition_2a:
- !Mc MS Mq MV c S1 S2.
-  P_sem Mc MS Mq MV (P_implements c S1) /\
-  P_sem Mc MS Mq MV (P_refines S1 S2) ==>
-  P_sem Mc MS Mq MV (P_implements c S2)
+ !omega Mc MS Mq MV c S1 S2.
+  P_sem omega Mc MS Mq MV (P_implements c S1) /\
+  P_sem omega Mc MS Mq MV (P_refines S1 S2) ==>
+  P_sem omega Mc MS Mq MV (P_implements c S2)
 Proof
  rw [P_sem] >> METIS_TAC [SUBSET_DEF]
 QED
 
 Theorem proposition_2b:
- !Mc MS Mq MV S1 S2 q.
-  (P_sem Mc MS Mq MV
+ !omega Mc MS Mq MV S1 S2 q.
+  (!s. MS s SUBSET POW omega) /\
+  (!s. MV s SUBSET POW omega) /\
+  (P_sem omega Mc MS Mq MV
    (P_forall_c q
     (P_implies 
      (P_implements (c_var q) S1)
      (P_implements (c_var q) S2)))) ==>
-  P_sem Mc MS Mq MV (P_refines S1 S2)
+  P_sem omega Mc MS Mq MV (P_refines S1 S2)
 Proof
- rw [P_sem,c_sem] >> METIS_TAC [SUBSET_DEF,APPLY_UPDATE_THM]
+ rw [P_sem,c_sem] >>
+ `S_sem omega MS MV S1 SUBSET POW omega`
+  by METIS_TAC [S_sem_omega] >>
+ METIS_TAC [SUBSET_DEF,APPLY_UPDATE_THM,IN_POW]
+QED
+
+Theorem proposition_2b_meta:
+ !omega Mc MS Mq MV S1 S2.
+  (!B. B IN S_sem omega MS MV S1 ==> B IN S_sem omega MS MV S2) ==>
+  P_sem omega Mc MS Mq MV (P_refines S1 S2)
+Proof
+ rw [S_sem,P_sem,SUBSET_DEF]
 QED
 
 Theorem proposition_3a:
- !Mc MS Mq MV S q1 q2.
+ !omega Mc MS Mq MV S q1 q2.
+  (!s. MS s SUBSET POW omega) /\
+  (!s. MV s SUBSET POW omega) /\
    q1 <> q2 ==>
-   (P_sem Mc MS Mq MV
+   (P_sem omega Mc MS Mq MV
     (P_forall_c q1 (P_forall_c q2
      (P_implies
       (P_implements (c_var q1) S)
       (P_implements (c_comp (c_var q1) (c_var q2)) S))))) ==>
-   P_sem Mc MS Mq MV (P_asserts S)
+   P_sem omega Mc MS Mq MV (P_asserts S)
 Proof
- rw [P_sem,c_sem,downward_closed] >>
+ rw [P_sem,c_sem,downward_closed] >> 
+ `e SUBSET omega` by METIS_TAC [IN_POW,SUBSET_DEF,S_sem_omega] >>
+ `e' SUBSET omega` by fs [SUBSET_DEF] >>
  METIS_TAC [INTER_SUBSET_EQN,APPLY_UPDATE_THM]
 QED
 
-Theorem proposition3_b:
- !Mc MS Mq MV S c1 c2.
-  P_sem Mc MS Mq MV (P_asserts S) /\
-  P_sem Mc MS Mq MV (P_implements c1 S) ==>
-  P_sem Mc MS Mq MV (P_implements (c_comp c1 c2) S)
+Theorem proposition_3a_meta:
+ !omega Mc MS Mq MV S.
+  (!B1 B2. B1 IN S_sem omega MS MV S ==> B1 INTER B2 IN S_sem omega MS MV S) ==>
+  P_sem omega Mc MS Mq MV (P_asserts S)
+Proof
+ rw [S_sem,P_sem,downward_closed] >>
+ METIS_TAC [INTER_SUBSET_EQN]
+QED
+
+Theorem proposition_3b:
+ !omega Mc MS Mq MV S c1 c2.
+  P_sem omega Mc MS Mq MV (P_asserts S) /\
+  P_sem omega Mc MS Mq MV (P_implements c1 S) ==>
+  P_sem omega Mc MS Mq MV (P_implements (c_comp c1 c2) S)
 Proof
  rw [P_sem,downward_closed,c_sem] >>
  METIS_TAC [INTER_SUBSET]
 QED
 
 Theorem proposition_4a:
- !Mc MS Mq MV S1 S2 c.
-  P_sem Mc MS Mq MV (P_implements c S1) /\
-  P_sem Mc MS Mq MV (P_implements c S2) ==>
-  P_sem Mc MS Mq MV (P_implements c (S_conj S1 S2))
+ !omega Mc MS Mq MV S1 S2 c.
+  P_sem omega Mc MS Mq MV (P_implements c S1) /\
+  P_sem omega Mc MS Mq MV (P_implements c S2) ==>
+  P_sem omega Mc MS Mq MV (P_implements c (S_conj S1 S2))
 Proof
  rw [P_sem,S_sem]
 QED
 
 Theorem proposition_4b:
- !Mc MS Mq MV S1 S2 c.
-  P_sem Mc MS Mq MV (P_implements c (S_conj S1 S2)) ==>
-  P_sem Mc MS Mq MV (P_implements c S1)
+ !omega Mc MS Mq MV S1 S2 c.
+  P_sem omega Mc MS Mq MV (P_implements c (S_conj S1 S2)) ==>
+  P_sem omega Mc MS Mq MV (P_implements c S1)
 Proof
  rw [P_sem,S_sem]
 QED
 
 Theorem proposition_4b_alt:
- !Mc MS Mq MV S1 S2 c.
-  P_sem Mc MS Mq MV (P_implements c (S_conj S1 S2)) ==>
-  P_sem Mc MS Mq MV (P_implements c S2)
+ !omega Mc MS Mq MV S1 S2 c.
+  P_sem omega Mc MS Mq MV (P_implements c (S_conj S1 S2)) ==>
+  P_sem omega Mc MS Mq MV (P_implements c S2)
 Proof
  rw [P_sem,S_sem]
 QED
 
 Theorem proposition_5a:
- !Mc MS Mq MV S1 S2 c q1 q2.
-  q1 <> q2 ==>
-  fv_c c = {} ==>
-  P_sem Mc MS Mq MV (P_implements c (S_par S1 S2)) ==>
-  P_sem Mc MS Mq MV 
+ !omega Mc MS Mq MV S1 S2 c q1 q2.
+  (!s. MS s SUBSET POW omega) /\
+  (!s. MV s SUBSET POW omega) /\
+  q1 <> q2 /\
+  q1 NOTIN fv_c c /\
+  q2 NOTIN fv_c c ==>
+  P_sem omega Mc MS Mq MV (P_implements c (S_par S1 S2)) ==>
+  P_sem omega Mc MS Mq MV 
    (P_exists_c q1 (P_exists_c q2
      (P_and (P_implements (c_var q1) S1)
       (P_and (P_implements (c_var q2) S2)
@@ -384,115 +516,1079 @@ Theorem proposition_5a:
 Proof
  rw [P_sem,c_sem,S_sem,double_intersection,APPLY_UPDATE_THM] >>
  Q.EXISTS_TAC `a` >>
+ rw [] >- METIS_TAC [IN_POW,SUBSET_DEF,S_sem_omega] >>
  Q.EXISTS_TAC `b` >>
- rw [] >>
- METIS_TAC [fv_c_empty_c_sem]
+ rw [] >- METIS_TAC [IN_POW,SUBSET_DEF,S_sem_omega] >>
+ METIS_TAC [fv_c_notin_c_sem] 
+QED
+
+Theorem proposition_5a_meta:
+ !omega Mc MS Mq MV S1 S2 c.
+  P_sem omega Mc MS Mq MV (P_implements c (S_par S1 S2)) ==>
+  ?B1 B2. B1 IN S_sem omega MS MV S1 /\
+   B2 IN S_sem omega MS MV S2 /\
+   B1 INTER B2 = c_sem Mc Mq c
+Proof
+ rw [P_sem,S_sem,double_intersection] >>
+ Q.EXISTS_TAC `a` >> Q.EXISTS_TAC `b` >>
+ rw []
 QED
 
 Theorem proposition_5b:
- !Mc MS Mq MV S1 S2 c1 c2.
-  P_sem Mc MS Mq MV (P_implements c1 S1) /\
-  P_sem Mc MS Mq MV (P_implements c2 S2) ==>
-  P_sem Mc MS Mq MV (P_implements (c_comp c1 c2) (S_par S1 S2))
+ !omega Mc MS Mq MV S1 S2 c1 c2.
+  P_sem omega Mc MS Mq MV (P_implements c1 S1) /\
+  P_sem omega Mc MS Mq MV (P_implements c2 S2) ==>
+  P_sem omega Mc MS Mq MV (P_implements (c_comp c1 c2) (S_par S1 S2))
 Proof
  rw [P_sem,c_sem,S_sem,double_intersection] >> METIS_TAC []
 QED
 
 Theorem proposition_6a:
- !Mc MS Mq MV S1 S2. P_sem Mc MS Mq MV (P_refines (S_conj S1 S2) (S_par S1 S2))
+ !omega Mc MS Mq MV S1 S2.
+  P_sem omega Mc MS Mq MV (P_refines (S_conj S1 S2) (S_par S1 S2))
 Proof
  rw [P_sem,S_sem,double_intersection,SUBSET_DEF] >> METIS_TAC [INTER_IDEMPOT]
 QED
 
 Theorem proposition_6b:
- !Mc MS Mq MV S1 S2.
-  P_sem Mc MS Mq MV (P_asserts S1) /\ P_sem Mc MS Mq MV (P_asserts S2) ==>
-  P_sem Mc MS Mq MV (P_refines (S_par S1 S2) (S_conj S1 S2))
+ !omega Mc MS Mq MV S1 S2.
+  P_sem omega Mc MS Mq MV (P_asserts S1) /\ P_sem omega Mc MS Mq MV (P_asserts S2) ==>
+  P_sem omega Mc MS Mq MV (P_refines (S_par S1 S2) (S_conj S1 S2))
 Proof
  rw [P_sem,S_sem,downward_closed,double_intersection,SUBSET_DEF] >>
  METIS_TAC [SUBSET_DEF,INTER_SUBSET]
 QED
 
 Theorem proposition_7a:
- !Mc MS Mq MV S1 S2. P_sem Mc MS Mq MV (P_refines (S_par S1 (S_assume S1 S2)) S2)
+ !omega Mc MS Mq MV S1 S2.
+  P_sem omega Mc MS Mq MV (P_refines (S_par S1 (S_assume S1 S2)) S2)
 Proof
  rw [P_sem,S_sem,double_intersection,SUBSET_DEF] >> METIS_TAC [INTER_COMM]
 QED
 
 Theorem proposition_7a_alt:
- !Mc MS Mq MV S1 S2 c1 c2.
-  P_sem Mc MS Mq MV (P_implements c1 S1) /\
-  P_sem Mc MS Mq MV (P_implements c2 (S_assume S1 S2)) ==>
-  P_sem Mc MS Mq MV (P_implements (c_comp c1 c2) S2)
+ !omega Mc MS Mq MV S1 S2 c1 c2.
+  P_sem omega Mc MS Mq MV (P_implements c1 S1) /\
+  P_sem omega Mc MS Mq MV (P_implements c2 (S_assume S1 S2)) ==>
+  P_sem omega Mc MS Mq MV (P_implements (c_comp c1 c2) S2)
 Proof
  rw [P_sem,c_sem,S_sem] >> METIS_TAC [INTER_COMM]
 QED
 
 Theorem proposition_7b:
- !Mc MS Mq MV S1 S2 c2 q1.
+ !omega Mc MS Mq MV S1 S2 c2 q1.
+  (!s. Mc s SUBSET omega) /\
+  (!s. Mq s SUBSET omega) /\
+  (!s. MS s SUBSET POW omega) /\
+  (!s. MV s SUBSET POW omega) /\  
    q1 NOTIN fv_c c2 ==>
-   (P_sem Mc MS Mq MV
+   (P_sem omega Mc MS Mq MV
     (P_forall_c q1
      (P_implies (P_implements (c_var q1) S1)
       (P_implements (c_comp (c_var q1) c2) S2)))) ==>
-   P_sem Mc MS Mq MV (P_implements c2 (S_assume S1 S2))
+   P_sem omega Mc MS Mq MV (P_implements c2 (S_assume S1 S2))
 Proof
- rw [P_sem,c_sem,S_sem,APPLY_UPDATE_THM] >>
- `(b' INTER c_sem Mc Mq c2) IN S_sem MS MV S2` suffices_by METIS_TAC [INTER_COMM] >>
- `c_sem Mc Mq c2 = c_sem Mc ((q1 =+ b') Mq) c2`
-  suffices_by METIS_TAC [] >>
+ rw [P_sem,c_sem,S_sem,APPLY_UPDATE_THM] >-
+ METIS_TAC [IN_POW,c_sem_omega] >>
+ `(B' INTER c_sem Mc Mq c2) IN S_sem omega MS MV S2` suffices_by METIS_TAC [INTER_COMM] >>
+ `c_sem Mc Mq c2 = c_sem Mc ((q1 =+ B') Mq) c2`
+  suffices_by METIS_TAC [IN_POW,SUBSET_DEF,S_sem_omega] >>
  match_mp_tac fv_c_eq_c_sem >>
  rw [APPLY_UPDATE_THM] >> fs []
 QED
 
-Theorem proposition_7b_alt:
- !Mc MS Mq MV S1 S2 c2. 
-  P_sem Mc MS Mq MV (P_implements c2 S2) ==>
-  P_sem Mc MS Mq MV (P_asserts S2) ==>
-  P_sem Mc MS Mq MV (P_implements c2 (S_assume S1 S2))
+Theorem proposition_7b_meta:
+ !omega Mc MS Mq MV S1 S2 c2.
+  (!s. Mc s SUBSET omega) /\
+  (!s. Mq s SUBSET omega) /\
+  (!B. B IN S_sem omega MS MV S1 ==> B INTER c_sem Mc Mq c2 IN S_sem omega MS MV S2) ==>
+  P_sem omega Mc MS Mq MV (P_implements c2 (S_assume S1 S2))
 Proof
- rw [P_sem,S_sem,downward_closed] >>
+ rw [P_sem,S_sem,c_sem] >-
+ METIS_TAC [IN_POW,c_sem_omega] >>
+ METIS_TAC [INTER_COMM]
+QED
+
+Theorem proposition_7b_alt:
+ !omega Mc MS Mq MV S1 S2 c2.
+  (!s. Mc s SUBSET omega) /\
+  (!s. Mq s SUBSET omega) /\
+  P_sem omega Mc MS Mq MV (P_implements c2 S2) /\
+  P_sem omega Mc MS Mq MV (P_asserts S2) ==>
+  P_sem omega Mc MS Mq MV (P_implements c2 (S_assume S1 S2))
+Proof
+ rw [P_sem,S_sem,downward_closed] >-
+ METIS_TAC [IN_POW,c_sem_omega] >>
  METIS_TAC [INTER_SUBSET]
 QED
 
-Theorem proposition_8:
- !MS MV S. S_sem MS MV S = S_sem MS MV (S_assume S_top S)
+Theorem proposition_8_meta:
+ !omega MS MV S.
+  (!s. MS s SUBSET POW omega) /\
+  (!s. MV s SUBSET POW omega) ==>
+  S_sem omega MS MV S = S_sem omega MS MV (S_assume (S_const Sc_top) S)
 Proof
- rw [S_sem]
+ rw [S_sem,EXTENSION] >> EQ_TAC >> rw [] >| [
+  METIS_TAC [SUBSET_DEF,S_sem_omega],
+
+  `omega SUBSET B'` by METIS_TAC [SUBSET_DEF] >>
+  `x INTER B' = x` suffices_by METIS_TAC [IN_POW] >>
+  METIS_TAC [SUBSET_DEF,SUBSET_INTER_ABSORPTION,IN_POW,S_sem_omega],
+
+  `x SUBSET omega` by METIS_TAC [IN_POW] >>
+  `x INTER omega = x` by METIS_TAC [SUBSET_INTER_ABSORPTION] >>
+  METIS_TAC []
+ ]
+QED
+
+Theorem proposition_8:
+ !omega Mc MS Mq MV S.
+  (!s. MS s SUBSET POW omega) /\
+  (!s. MV s SUBSET POW omega) ==>
+  P_sem omega Mc MS Mq MV (P_S_eq S (S_assume (S_const Sc_top) S))
+Proof
+ rw [P_sem] >> METIS_TAC [proposition_8_meta]
 QED
 
 Theorem proposition_9:
- !Mc MS Mq MV S1 S2.
-  P_sem Mc MS Mq MV (P_asserts S2) ==>
-  P_sem Mc MS Mq MV (P_asserts (S_assume S1 S2))
+ !omega Mc MS Mq MV S1 S2.
+  P_sem omega Mc MS Mq MV (P_asserts S2) ==>
+  P_sem omega Mc MS Mq MV (P_asserts (S_assume S1 S2))
 Proof
- rw [P_sem,downward_closed,S_sem] >>
- `e INTER b' IN S_sem MS MV S2` by METIS_TAC [] >>
- `e' INTER b' SUBSET e INTER b'` suffices_by METIS_TAC [] >>
+ rw [P_sem,downward_closed,S_sem] >-
+ METIS_TAC [IN_POW,SUBSET_DEF] >>
+ `e INTER B' IN S_sem omega MS MV S2` by METIS_TAC [] >>
+ `e' INTER B' SUBSET e INTER B'` suffices_by METIS_TAC [] >>
  fs [SUBSET_DEF]
 QED
 
 Theorem compat_comp:
- !Mc MS Mq MV c1 c2.
-  P_sem Mc MS Mq MV (P_implements (c_comp c1 c2) S_compat) <=>
-  (c_sem Mc Mq c1) INTER (c_sem Mc Mq c2) <> {}
+ !omega Mc MS Mq MV c1 c2.
+  (!s. Mc s SUBSET omega) /\
+  (!s. Mq s SUBSET omega) ==>
+  (P_sem omega Mc MS Mq MV (P_implements (c_comp c1 c2) (S_const Sc_compat)) <=>
+  (c_sem Mc Mq c1) INTER (c_sem Mc Mq c2) <> {})
 Proof
- rw [] >> EQ_TAC >> rw [P_sem,c_sem,S_sem]
+ rw [] >> EQ_TAC >> rw [P_sem,c_sem,S_sem] >> 
+ METIS_TAC [IN_POW,SUBSET_DEF,IN_INTER,c_sem_omega]
 QED
 
-Theorem spec_holds_system_sound:
- !Mc MS Mq MV. spec_system_sound spec_holds Mc MS Mq MV
+(* c substitution *)
+
+Theorem csubst_c_triv:
+ !c. csubst_c c_var c = c
 Proof
- strip_tac >> strip_tac >> strip_tac >> strip_tac >>
- `!G P. spec_holds G P ==> 
-   (!P0. P0 IN G ==> P_sem Mc MS Mq MV P0) ==> P_sem Mc MS Mq MV P`
+ Induct >> rw [csubst_c]
+QED
+
+Theorem csubst_c_valuation:
+ !c Mq1 Mq2. (!x. x IN fv_c c ==> (Mq1 x = Mq2 x)) ==> (csubst_c Mq1 c = csubst_c Mq2 c)
+Proof
+ Induct >> rw [csubst_c,fv_c]
+QED
+
+Theorem csubst_c_fv_c:
+ !c Mq. fv_c (csubst_c Mq c) = { x | ?y. y IN fv_c c /\ x IN fv_c (Mq y) }
+Proof
+ Induct >> rw [csubst_c,fv_c] >>
+ rw [UNION_DEF,EXTENSION] >> METIS_TAC []
+QED
+
+Theorem csubst_P_triv:
+ !P. csubst_P c_var P = P
+Proof
+ Induct >> rw [csubst_P,fv_P_c] >>
+ fs [combinTheory.APPLY_UPDATE_ID,fv_c] >>
+ rw [csubst_c_triv]
+QED
+
+Theorem csubst_P_valuation:
+ !P Mq1 Mq2. (!x. x IN fv_P_c P ==> (Mq1 x = Mq2 x)) ==>
+  (csubst_P Mq1 P = csubst_P Mq2 P)
+Proof
+ Induct >> rw [fv_P_c,csubst_P] >>
+ fs [combinTheory.UPDATE_APPLY,fv_P_c,fv_c] >>
+ rw [csubst_c_valuation] >| [
+  `csubst_P ((s =+ c_var s) Mq1) P = csubst_P ((s =+ c_var s) Mq2) P`
+   by fs[combinTheory.APPLY_UPDATE_THM] >>
+  rw [],
+
+  `csubst_P ((s =+ c_var s) Mq1) P = csubst_P ((s =+ c_var s) Mq2) P`
+   by fs[combinTheory.APPLY_UPDATE_THM] >>
+  rw [combinTheory.APPLY_UPDATE_THM],
+
+  fs[combinTheory.APPLY_UPDATE_THM] >>
+  Cases_on `s = y` >> fs [fv_c] >>
+  METIS_TAC [],
+
+  fs[combinTheory.APPLY_UPDATE_THM] >>
+  Cases_on `s = y` >> fs [fv_c] >>
+  METIS_TAC [],
+
+  fs[combinTheory.APPLY_UPDATE_THM] >>
+  Cases_on `s = y` >> fs [fv_c] >>
+  METIS_TAC [],
+
+  fs[combinTheory.APPLY_UPDATE_THM] >>
+  Cases_on `s = y` >> fs [fv_c] >>
+  METIS_TAC [],
+
+  fs[combinTheory.APPLY_UPDATE_THM],
+
+  `csubst_P ((s =+ c_var s) Mq1) P = csubst_P ((s =+ c_var s) Mq2) P`
+   by fs[combinTheory.APPLY_UPDATE_THM] >>
+  rw [combinTheory.APPLY_UPDATE_THM],
+
+  `csubst_P ((s =+ c_var s) Mq1) P = csubst_P ((s =+ c_var s) Mq2) P`
+   by fs[combinTheory.APPLY_UPDATE_THM] >>
+  rw [combinTheory.APPLY_UPDATE_THM],
+
+  fs[combinTheory.APPLY_UPDATE_THM] >>
+  Cases_on `s = y` >> fs [fv_c] >>
+  METIS_TAC [],
+
+  fs[combinTheory.APPLY_UPDATE_THM] >>
+  Cases_on `s = y` >> fs [fv_c] >>
+  METIS_TAC [],
+
+  fs[combinTheory.APPLY_UPDATE_THM] >>
+  Cases_on `s = y` >> fs [fv_c] >>
+  METIS_TAC [],
+
+  fs[combinTheory.APPLY_UPDATE_THM] >>
+  Cases_on `s = y` >> fs [fv_c] >>
+  METIS_TAC [],
+
+  `csubst_P ((s =+ c_var s) Mq1) P = csubst_P ((s =+ c_var s) Mq2) P`
+   by fs[combinTheory.APPLY_UPDATE_THM] >>
+  rw [combinTheory.APPLY_UPDATE_THM]
+ ]
+QED
+
+(* S substitution *)
+
+Theorem Ssubst_S_triv:
+ !S. Ssubst_S S_var S = S
+Proof
+ Induct >> rw [Ssubst_S]
+QED
+
+Theorem Ssubst_S_valuation:
+ !c MV1 MV2. (!x. x IN fv_S c ==> (MV1 x = MV2 x)) ==> (Ssubst_S MV1 c = Ssubst_S MV2 c)
+Proof
+ Induct >> rw [Ssubst_S,fv_S]
+QED
+
+Theorem Ssubst_S_fv_S:
+ !S MV. fv_S (Ssubst_S MV S) = { x | ?y. y IN fv_S S /\ x IN fv_S (MV y) }
+Proof
+ Induct >> rw [Ssubst_S,fv_S] >>
+ rw [UNION_DEF,EXTENSION] >> METIS_TAC []
+QED
+
+Theorem Ssubst_P_triv:
+ !P. Ssubst_P S_var P = P
+Proof
+ Induct >> rw [Ssubst_P,fv_P_S] >>
+ fs [combinTheory.APPLY_UPDATE_ID,fv_S] >>
+ rw [Ssubst_S_triv]
+QED
+
+Theorem Ssubst_P_valuation:
+ !P MV1 MV2. (!x. x IN fv_P_S P ==> (MV1 x = MV2 x)) ==>
+  (Ssubst_P MV1 P = Ssubst_P MV2 P)
+Proof
+ Induct >> rw [fv_P_S,Ssubst_P] >>
+ fs [combinTheory.UPDATE_APPLY,fv_P_S,fv_S] >>
+ rw [Ssubst_S_valuation] >| [
+  `Ssubst_P ((s =+ S_var s) MV1) P = Ssubst_P ((s =+ S_var s) MV2) P`
+   by fs[combinTheory.APPLY_UPDATE_THM] >>
+  rw [],
+
+  `Ssubst_P ((s =+ S_var s) MV1) P = Ssubst_P ((s =+ S_var s) MV2) P`
+   by fs[combinTheory.APPLY_UPDATE_THM] >>
+  rw [combinTheory.APPLY_UPDATE_THM],
+
+  fs[combinTheory.APPLY_UPDATE_THM] >>
+  Cases_on `s = y` >> fs [fv_S] >>
+  METIS_TAC [],
+
+  fs[combinTheory.APPLY_UPDATE_THM] >>
+  Cases_on `s = y` >> fs [fv_S] >>
+  METIS_TAC [],
+
+  fs[combinTheory.APPLY_UPDATE_THM] >>
+  Cases_on `s = y` >> fs [fv_S] >>
+  METIS_TAC [],
+
+  fs[combinTheory.APPLY_UPDATE_THM] >>
+  Cases_on `s = y` >> fs [fv_S] >>
+  METIS_TAC [],
+
+  fs[combinTheory.APPLY_UPDATE_THM],
+
+  `Ssubst_P ((s =+ S_var s) MV1) P = Ssubst_P ((s =+ S_var s) MV2) P`
+   by fs[combinTheory.APPLY_UPDATE_THM] >>
+  rw [combinTheory.APPLY_UPDATE_THM],
+
+  `Ssubst_P ((s =+ S_var s) MV1) P = Ssubst_P ((s =+ S_var s) MV2) P`
+   by fs[combinTheory.APPLY_UPDATE_THM] >>
+  rw [combinTheory.APPLY_UPDATE_THM],
+
+  fs[combinTheory.APPLY_UPDATE_THM] >>
+  Cases_on `s = y` >> fs [fv_S] >>
+  METIS_TAC [],
+
+  fs[combinTheory.APPLY_UPDATE_THM] >>
+  Cases_on `s = y` >> fs [fv_S] >>
+  METIS_TAC [],
+
+  fs[combinTheory.APPLY_UPDATE_THM] >>
+  Cases_on `s = y` >> fs [fv_S] >>
+  METIS_TAC [],
+
+  fs[combinTheory.APPLY_UPDATE_THM] >>
+  Cases_on `s = y` >> fs [fv_S] >>
+  METIS_TAC [],
+
+  `Ssubst_P ((s =+ S_var s) MV1) P = Ssubst_P ((s =+ S_var s) MV2) P`
+   by fs[combinTheory.APPLY_UPDATE_THM] >>
+  rw [combinTheory.APPLY_UPDATE_THM]
+ ]
+QED
+
+(* free variables *)
+
+Theorem FINITE_fv_c:
+ !c. FINITE (fv_c c)
+Proof
+ Induct >> rw [fv_c]
+QED
+
+Theorem FINITE_fv_P_c:
+ !P. FINITE (fv_P_c P)
+Proof
+ Induct >> rw [fv_P_c,FINITE_fv_c]
+QED
+
+Theorem FINITE_fv_S:
+ !c. FINITE (fv_S c)
+Proof
+ Induct >> rw [fv_S]
+QED
+
+Theorem FINITE_fv_P_S:
+ !P. FINITE (fv_P_S P)
+Proof
+ Induct >> rw [fv_P_S,FINITE_fv_S]
+QED
+
+Theorem SVARIANT_fv_P_c:
+ !P. SVARIANT (fv_P_c P) NOTIN fv_P_c P
+Proof
+ METIS_TAC [SVARIANT_FINITE,FINITE_fv_P_c]
+QED
+
+Theorem SVARIANT_fv_P_S:
+ !P. SVARIANT (fv_P_S P) NOTIN fv_P_S P
+Proof
+ METIS_TAC [SVARIANT_FINITE,FINITE_fv_P_S]
+QED
+
+Theorem c_sem_csubst:
+ !c Mc Mq qc.
+  c_sem Mc Mq (csubst_c qc c) = c_sem Mc (c_sem Mc Mq o qc) c
+Proof
+ Induct_on `c` >> rw [c_sem,csubst_c]
+QED
+
+Theorem c_sem_csubst1:
+ !c Mc Mq c' q.
+  c_sem Mc ((q =+ c_sem Mc Mq c') Mq) c =
+  c_sem Mc Mq (csubst_c ((q =+ c') c_var) c)
+Proof
+ Induct >> rw [c_sem,csubst_c] >>
+ fs[combinTheory.APPLY_UPDATE_THM] >>
+ Cases_on `q = s` >> rw [c_sem]
+QED
+
+Theorem S_sem_Ssubst:
+ !S omega MS MV VS.
+  S_sem omega MS MV (Ssubst_S VS S) = S_sem omega MS (S_sem omega MS MV o VS) S
+Proof
+ ho_match_mp_tac S_induction >> rw [S_sem,Ssubst_S] >>
+ Cases_on `S'` >> rw [S_sem]
+QED
+
+Theorem S_sem_Ssubst1:
+ !S omega MS MV S' V.
+  S_sem omega MS ((V =+ S_sem omega MS MV S') MV) S =
+  S_sem omega MS MV (Ssubst_S ((V =+ S') S_var) S)
+Proof
+ Induct >> rw [S_sem,Ssubst_S] >>
+ fs[combinTheory.APPLY_UPDATE_THM] >>
+ Cases_on `V = s` >> rw [S_sem] >>
+ Cases_on `S'` >> rw [S_sem]
+QED
+
+Theorem fv_P_c_IN_UNION:
+ !P qc s. 
+ {x | (∃y'. y' ∈ fv_P_c P ∧ x ∈ fv_c (if s = y' then c_var y' else qc y'))} =
+ ({ x | s IN fv_P_c P /\ x IN fv_c (c_var s) } UNION
+  { x | ?y. y IN fv_P_c P /\ y <> s /\ x IN fv_c (qc y) })
+Proof
+ rw [EXTENSION] >> EQ_TAC >> rw [] >> Cases_on `s = y'` >> rw [] >> fs [fv_c] >| [
+   METIS_TAC [],
+   
+   rw [] >> Q.EXISTS_TAC `s` >> rw [fv_c],
+
+   rw [] >> Q.EXISTS_TAC `s` >> rw [fv_c],
+
+   Q.EXISTS_TAC `y` >> rw [],
+
+   Q.EXISTS_TAC `y` >> rw []
+ ]
+QED
+
+Theorem fv_P_S_IN_UNION:
+ !P VS s. 
+ {x | (∃y'. y' ∈ fv_P_S P ∧ x IN fv_S (if s = y' then S_var y' else VS y'))} =
+ ({ x | s IN fv_P_S P /\ x IN fv_S (S_var s) } UNION
+  { x | ?y. y IN fv_P_S P /\ y <> s /\ x IN fv_S (VS y) })
+Proof
+ rw [EXTENSION] >> EQ_TAC >> rw [] >> Cases_on `s = y'` >> rw [] >> fs [fv_S] >| [
+   METIS_TAC [],
+   
+   rw [] >> Q.EXISTS_TAC `s` >> rw [fv_S],
+
+   rw [] >> Q.EXISTS_TAC `s` >> rw [fv_S],
+
+   Q.EXISTS_TAC `y` >> rw [],
+
+   Q.EXISTS_TAC `y` >> rw []
+ ]
+QED
+
+Theorem fv_P_c_BIGUNION:
+ !P qc. 
+ { x | ?y. y IN fv_P_c P /\ x IN fv_c (qc y) } =
+  BIGUNION (IMAGE (\y. fv_c (qc y)) (fv_P_c P))
+Proof
+ rw [BIGUNION_IMAGE]
+QED
+
+Theorem fv_P_S_BIGUNION:
+ !P VS. 
+ { x | ?y. y IN fv_P_S P /\ x IN fv_S (VS y) } =
+  BIGUNION (IMAGE (\y. fv_S (VS y)) (fv_P_S P))
+Proof
+ rw [BIGUNION_IMAGE]
+QED
+
+Theorem FINITE_fv_P_c_BIGUNION:
+ !P qc. FINITE { x | ?y. y IN fv_P_c P /\ x IN fv_c (qc y) }
+Proof
+ rw [fv_P_c_BIGUNION] >-
+ METIS_TAC [IMAGE_FINITE,FINITE_fv_P_c] >>
+ METIS_TAC [FINITE_fv_c]
+QED
+
+Theorem FINITE_fv_P_S_BIGUNION:
+ !P VS. FINITE { x | ?y. y IN fv_P_S P /\ x IN fv_S (VS y) }
+Proof
+ rw [fv_P_S_BIGUNION] >-
+ METIS_TAC [IMAGE_FINITE,FINITE_fv_P_S] >>
+ METIS_TAC [FINITE_fv_S]
+QED
+
+Theorem FINITE_fv_P_c_SUBSET:
+ !P qc s. FINITE { x | ?y. y IN fv_P_c P /\ y <> s /\ x IN fv_c (qc y) }
+Proof
+ rw [] >>
+ `{ x | ?y. y IN fv_P_c P /\ y <> s /\ x IN fv_c (qc y) } SUBSET
+  { x | ?y. y IN fv_P_c P /\ x IN fv_c (qc y) }`
+ suffices_by METIS_TAC [SUBSET_FINITE,FINITE_fv_P_c_BIGUNION] >>
+ rw [SUBSET_DEF] >> METIS_TAC []
+QED
+
+Theorem FINITE_fv_P_S_SUBSET:
+ !P VS s. FINITE { x | ?y. y IN fv_P_S P /\ y <> s /\ x IN fv_S (VS y) }
+Proof
+ rw [] >>
+ `{ x | ?y. y IN fv_P_S P /\ y <> s /\ x IN fv_S (VS y) } SUBSET
+  { x | ?y. y IN fv_P_S P /\ x IN fv_S (VS y) }`
+ suffices_by METIS_TAC [SUBSET_FINITE,FINITE_fv_P_S_BIGUNION] >>
+ rw [SUBSET_DEF] >> METIS_TAC []
+QED
+
+Theorem FINITE_s_fv_P_c:
+ !P s. FINITE { x | s IN fv_P_c P /\ x IN fv_c (c_var s) }
+Proof
+ rw [] >>
+ `{x | s ∈ fv_P_c P ∧ x ∈ fv_c (c_var s)} SUBSET
+  fv_c (c_var s)`
+  suffices_by METIS_TAC [SUBSET_FINITE,FINITE_fv_c] >>
+ rw [SUBSET_DEF]
+QED
+
+Theorem FINITE_s_fv_P_S:
+ !P s. FINITE { x | s IN fv_P_S P /\ x IN fv_S (S_var s) }
+Proof
+ rw [] >>
+ `{x | s IN fv_P_S P ∧ x IN fv_S (S_var s)} SUBSET
+  fv_S (S_var s)`
+  suffices_by METIS_TAC [SUBSET_FINITE,FINITE_fv_S] >>
+ rw [SUBSET_DEF]
+QED
+
+Theorem FINITE_fv_P_c_fv_c:
+ !P qc s.
+  FINITE {x | (∃y'. y' ∈ fv_P_c P ∧ x ∈ fv_c (if s = y' then c_var y' else qc y'))}
+Proof
+ rw [fv_P_c_IN_UNION] >-
+ rw [FINITE_s_fv_P_c] >-
+ rw [FINITE_fv_P_c_SUBSET]
+QED
+
+Theorem FINITE_fv_P_S_fv_S:
+ !P VS s.
+  FINITE {x | (?y'. y' IN fv_P_S P /\ x IN fv_S (if s = y' then S_var y' else VS y'))}
+Proof
+ rw [fv_P_S_IN_UNION] >-
+ rw [FINITE_s_fv_P_S] >-
+ rw [FINITE_fv_P_S_SUBSET]
+QED
+
+Theorem csubst_P_fv_P_c:
+ !P qc. fv_P_c (csubst_P qc P) = { x | ?y. y IN fv_P_c P /\ x IN fv_c (qc y) }
+Proof
+ Induct >> rw [fv_P_c,csubst_P,fv_c] >| [
+  rw [csubst_c_fv_c],
+
+  fs [combinTheory.APPLY_UPDATE_THM,fv_c,fv_P_c] >>
+  Cases_on `s = y` >> fs [fv_c] >>
+  fs [EXTENSION] >> rw [] >> EQ_TAC >> rw [] >| [
+    Cases_on `s = y'` >> fs [fv_c] >> Q.EXISTS_TAC `y'` >> rw [],
+
+    Q.EXISTS_TAC `y'` >> rw [],
+    
+    strip_tac >>
+    sg `x IN {x | (∃y'. y' ∈ fv_P_c P ∧ x ∈ fv_c (if s = y' then c_var y' else qc y'))}` >-
+     (rw [] >> Q.EXISTS_TAC `y'` >> rw []) >>
+    METIS_TAC [SVARIANT_FINITE,FINITE_fv_P_c_fv_c]
+  ],
+
+  fs [combinTheory.APPLY_UPDATE_THM,fv_c,fv_P_c] >>
+  rw [EXTENSION] >>
+  EQ_TAC >> rw [] >| [
+   Cases_on `s = y` >> fs [fv_c] >>
+   Q.EXISTS_TAC `y` >> rw [],
+
+   Q.EXISTS_TAC `y` >> rw [],
+   
+   Q.PAT_X_ASSUM `!y. Q \/ R` (STRIP_ASSUME_TAC o (Q.SPECL [`y`])) >> rw [] >>
+   Cases_on `s = y` >> fs [] >>
+   METIS_TAC []
+  ],
+
+  fs [combinTheory.APPLY_UPDATE_THM,fv_c,fv_P_c] >>
+  Cases_on `s = y` >> fs [fv_c] >>
+  fs [EXTENSION] >> rw [] >> EQ_TAC >> rw [] >| [
+    Cases_on `s = y'` >> fs [fv_c] >> Q.EXISTS_TAC `y'` >> rw [],
+
+    Q.EXISTS_TAC `y'` >> rw [],
+    
+    strip_tac >>
+    sg `x IN {x | (∃y'. y' ∈ fv_P_c P ∧ x ∈ fv_c (if s = y' then c_var y' else qc y'))}` >-
+     (rw [] >> Q.EXISTS_TAC `y'` >> rw []) >>
+    METIS_TAC [SVARIANT_FINITE,FINITE_fv_P_c_fv_c]
+  ],
+
+  fs [combinTheory.APPLY_UPDATE_THM,fv_c,fv_P_c] >>
+  rw [EXTENSION] >>
+  EQ_TAC >> rw [] >| [
+   Cases_on `s = y` >> fs [fv_c] >>
+   Q.EXISTS_TAC `y` >> rw [],
+
+   Q.EXISTS_TAC `y` >> rw [],
+   
+   Q.PAT_X_ASSUM `!y. Q \/ R` (STRIP_ASSUME_TAC o (Q.SPECL [`y`])) >> rw [] >>
+   Cases_on `s = y` >> fs [] >>
+   METIS_TAC []
+  ],
+
+  rw [UNION_DEF,EXTENSION] >> EQ_TAC >> METIS_TAC [],
+
+  rw [UNION_DEF,EXTENSION] >> EQ_TAC >> METIS_TAC [],
+
+  rw [UNION_DEF,EXTENSION] >> EQ_TAC >> METIS_TAC [],
+
+  rw [csubst_c_fv_c,UNION_DEF,EXTENSION] >> EQ_TAC >> METIS_TAC []
+ ]
+QED
+
+Theorem Ssubst_P_fv_P_S:
+ !P VS. fv_P_S (Ssubst_P VS P) = { x | ?y. y IN fv_P_S P /\ x IN fv_S (VS y) }
+Proof
+ Induct >> rw [fv_P_S,Ssubst_P,fv_S] >| [
+  rw [Ssubst_S_fv_S],
+
+  rw [Ssubst_S_fv_S,UNION_DEF,EXTENSION] >> METIS_TAC [],
+
+  rw [Ssubst_S_fv_S,UNION_DEF,EXTENSION] >> METIS_TAC [],
+
+  fs [combinTheory.APPLY_UPDATE_THM,fv_S,fv_P_S] >>
+  Cases_on `s = y` >> fs [fv_S] >>
+  fs [EXTENSION] >> rw [] >> EQ_TAC >> rw [] >| [
+    Cases_on `s = y'` >> fs [fv_c] >> Q.EXISTS_TAC `y'` >> rw [] >> fs [fv_S],
+
+    Q.EXISTS_TAC `y'` >> rw [],
+    
+    strip_tac >>
+    sg `x IN {x | (?y'. y' IN fv_P_S P /\ x IN fv_S (if s = y' then S_var y' else VS y'))}` >-
+     (rw [] >> Q.EXISTS_TAC `y'` >> rw []) >>
+    METIS_TAC [SVARIANT_FINITE,FINITE_fv_P_S_fv_S]
+  ],
+
+  fs [combinTheory.APPLY_UPDATE_THM,fv_S,fv_P_S] >>
+  rw [EXTENSION] >>
+  EQ_TAC >> rw [] >| [
+   Cases_on `s = y` >> fs [fv_S] >>
+   Q.EXISTS_TAC `y` >> rw [],
+
+   Q.EXISTS_TAC `y` >> rw [],
+
+   Q.PAT_X_ASSUM `!y. Q \/ R` (STRIP_ASSUME_TAC o (Q.SPECL [`y`])) >> rw [] >>
+   Cases_on `s = y` >> fs [] >>
+   METIS_TAC []
+  ],
+
+  fs [combinTheory.APPLY_UPDATE_THM,fv_S,fv_P_S] >>
+  Cases_on `s = y` >> fs [fv_S] >>
+  fs [EXTENSION] >> rw [] >> EQ_TAC >> rw [] >| [
+    Cases_on `s = y'` >> fs [fv_S] >> Q.EXISTS_TAC `y'` >> rw [],
+
+    Q.EXISTS_TAC `y'` >> rw [],
+    
+    strip_tac >>
+    sg `x IN {x | (?y'. y' IN fv_P_S P /\ x IN fv_S (if s = y' then S_var y' else VS y'))}` >-
+     (rw [] >> Q.EXISTS_TAC `y'` >> rw []) >>
+    METIS_TAC [SVARIANT_FINITE,FINITE_fv_P_S_fv_S]
+  ],
+
+  fs [combinTheory.APPLY_UPDATE_THM,fv_S,fv_P_S] >>
+  rw [EXTENSION] >>
+  EQ_TAC >> rw [] >| [
+   Cases_on `s = y` >> fs [fv_S] >>
+   Q.EXISTS_TAC `y` >> rw [],
+
+   Q.EXISTS_TAC `y` >> rw [],
+
+   Q.PAT_X_ASSUM `!y. Q \/ R` (STRIP_ASSUME_TAC o (Q.SPECL [`y`])) >> rw [] >>
+   Cases_on `s = y` >> fs [] >>
+   METIS_TAC []
+  ],
+
+  rw [UNION_DEF,EXTENSION] >> EQ_TAC >> METIS_TAC [],
+
+  rw [UNION_DEF,EXTENSION] >> EQ_TAC >> METIS_TAC [],
+
+  rw [UNION_DEF,EXTENSION] >> EQ_TAC >> METIS_TAC [],
+
+  rw [Ssubst_S_fv_S,UNION_DEF,EXTENSION] >> EQ_TAC >> METIS_TAC []
+ ]
+QED
+
+Theorem P_sem_csubst:
+ !P omega Mc MS Mq MV qc.
+  P_sem omega Mc MS Mq MV (csubst_P qc P) <=>
+  P_sem omega Mc MS (c_sem Mc Mq o qc) MV P
+Proof
+ Induct_on `P` >> rw [P_sem,csubst_P,fv_P_c,fv_c] >| [
+  rw [c_sem_csubst],
+
+  fs [combinTheory.APPLY_UPDATE_THM] >>
+  Cases_on `s = y` >> fs [fv_c] >>
+  EQ_TAC >> rw [] >-
+   (`!q. q IN fv_P_c P ==> 
+    (c_sem Mc Mq⦇SVARIANT (fv_P_c (csubst_P qc⦇s ↦ c_var s⦈ P)) ↦ qs⦈ ∘
+      qc⦇s ↦ c_var (SVARIANT (fv_P_c (csubst_P qc⦇s ↦ c_var s⦈ P)))⦈) q =
+    ((c_sem Mc Mq ∘ qc)⦇s ↦ qs⦈) q`
+     suffices_by METIS_TAC [fv_P_c_eq_P_sem] >>
+    rw [combinTheory.APPLY_UPDATE_THM,c_sem] >>
+    `SVARIANT (fv_P_c (csubst_P qc⦇s ↦ c_var s⦈ P)) NOTIN fv_P_c (csubst_P qc⦇s ↦ c_var s⦈ P)`
+     by METIS_TAC [SVARIANT_fv_P_c] >>
+    irule fv_c_eq_c_sem >>
+    rw [] >>
+    fs [combinTheory.APPLY_UPDATE_THM] >> rw [] >>
+    `SVARIANT (fv_P_c (csubst_P qc⦇s ↦ c_var s⦈ P)) IN
+     fv_P_c (csubst_P qc⦇s ↦ c_var s⦈ P)` suffices_by METIS_TAC [] >>
+    `fv_c (qc q) SUBSET fv_P_c (csubst_P qc⦇s ↦ c_var s⦈ P)`
+     suffices_by METIS_TAC [SUBSET_DEF] >>
+    rw [SUBSET_DEF] >>
+    rw [csubst_P_fv_P_c] >>
+    Q.EXISTS_TAC `q` >>
+    rw [combinTheory.APPLY_UPDATE_THM]) >>
+  `!q. q IN fv_P_c P ==> 
+  (c_sem Mc Mq⦇SVARIANT (fv_P_c (csubst_P qc⦇s ↦ c_var s⦈ P)) ↦ qs⦈ ∘
+     qc⦇s ↦ c_var (SVARIANT (fv_P_c (csubst_P qc⦇s ↦ c_var s⦈ P)))⦈) q =
+  ((c_sem Mc Mq ∘ qc)⦇s ↦ qs⦈) q`
+    suffices_by METIS_TAC [fv_P_c_eq_P_sem] >>
+  rw [combinTheory.APPLY_UPDATE_THM,c_sem] >>
+  `SVARIANT (fv_P_c (csubst_P qc⦇s ↦ c_var s⦈ P)) NOTIN fv_P_c (csubst_P qc⦇s ↦ c_var s⦈ P)`
+    by METIS_TAC [SVARIANT_fv_P_c] >>
+  irule fv_c_eq_c_sem >>
+  rw [] >>
+  fs [combinTheory.APPLY_UPDATE_THM] >> rw [] >>
+  `SVARIANT (fv_P_c (csubst_P qc⦇s ↦ c_var s⦈ P)) IN
+   fv_P_c (csubst_P qc⦇s ↦ c_var s⦈ P)` suffices_by METIS_TAC [] >>
+  `fv_c (qc q) SUBSET fv_P_c (csubst_P qc⦇s ↦ c_var s⦈ P)`
+    suffices_by METIS_TAC [SUBSET_DEF] >>
+  rw [SUBSET_DEF] >>
+  rw [csubst_P_fv_P_c] >>
+  Q.EXISTS_TAC `q` >>
+  rw [combinTheory.APPLY_UPDATE_THM],
+
+  fs [combinTheory.APPLY_UPDATE_THM] >>
+  EQ_TAC >> rw [] >-
+   (`!q. q IN fv_P_c P ==> (c_sem Mc Mq⦇s ↦ qs⦈ ∘ qc⦇s ↦ c_var s⦈) q = ((c_sem Mc Mq ∘ qc)⦇s ↦ qs⦈) q`
+    suffices_by METIS_TAC [fv_P_c_eq_P_sem] >>
+    rw [] >>
+    Q.PAT_X_ASSUM `!y. Q \/ R` (STRIP_ASSUME_TAC o (Q.SPECL [`q`])) >-
+     (rw [combinTheory.APPLY_UPDATE_THM,c_sem]) >>
+    Cases_on `s = q` >> fs [combinTheory.APPLY_UPDATE_THM,fv_c] >>
+    METIS_TAC [fv_c_notin_c_sem]) >>
+  `!q. q IN fv_P_c P ==> (c_sem Mc Mq⦇s ↦ qs⦈ ∘ qc⦇s ↦ c_var s⦈) q = ((c_sem Mc Mq ∘ qc)⦇s ↦ qs⦈) q`
+    suffices_by METIS_TAC [fv_P_c_eq_P_sem] >>
+  rw [] >>
+  Q.PAT_X_ASSUM `!y. Q \/ R` (STRIP_ASSUME_TAC o (Q.SPECL [`q`])) >-
+   (rw [combinTheory.APPLY_UPDATE_THM,c_sem]) >>
+  Cases_on `s = q` >> fs [combinTheory.APPLY_UPDATE_THM,fv_c] >>
+  METIS_TAC [fv_c_notin_c_sem],
+
+  fs [combinTheory.APPLY_UPDATE_THM] >>
+  Cases_on `s = y` >> fs [fv_c] >>
+  EQ_TAC >> rw [] >-
+   (`!q. q IN fv_P_c P ==> 
+    (c_sem Mc Mq⦇SVARIANT (fv_P_c (csubst_P qc⦇s ↦ c_var s⦈ P)) ↦ qs⦈ ∘
+      qc⦇s ↦ c_var (SVARIANT (fv_P_c (csubst_P qc⦇s ↦ c_var s⦈ P)))⦈) q =
+    ((c_sem Mc Mq ∘ qc)⦇s ↦ qs⦈) q`
+     suffices_by METIS_TAC [fv_P_c_eq_P_sem] >>
+    rw [combinTheory.APPLY_UPDATE_THM,c_sem] >>
+    `SVARIANT (fv_P_c (csubst_P qc⦇s ↦ c_var s⦈ P)) NOTIN fv_P_c (csubst_P qc⦇s ↦ c_var s⦈ P)`
+     by METIS_TAC [SVARIANT_fv_P_c] >>
+    irule fv_c_eq_c_sem >>
+    rw [] >>
+    fs [combinTheory.APPLY_UPDATE_THM] >> rw [] >>
+    `SVARIANT (fv_P_c (csubst_P qc⦇s ↦ c_var s⦈ P)) IN
+     fv_P_c (csubst_P qc⦇s ↦ c_var s⦈ P)` suffices_by METIS_TAC [] >>
+    `fv_c (qc q) SUBSET fv_P_c (csubst_P qc⦇s ↦ c_var s⦈ P)`
+     suffices_by METIS_TAC [SUBSET_DEF] >>
+    rw [SUBSET_DEF] >>
+    rw [csubst_P_fv_P_c] >>
+    Q.EXISTS_TAC `q` >>
+    rw [combinTheory.APPLY_UPDATE_THM]) >>
+  `!q. q IN fv_P_c P ==> 
+  (c_sem Mc Mq⦇SVARIANT (fv_P_c (csubst_P qc⦇s ↦ c_var s⦈ P)) ↦ qs⦈ ∘
+     qc⦇s ↦ c_var (SVARIANT (fv_P_c (csubst_P qc⦇s ↦ c_var s⦈ P)))⦈) q =
+  ((c_sem Mc Mq ∘ qc)⦇s ↦ qs⦈) q`
+    suffices_by METIS_TAC [fv_P_c_eq_P_sem] >>
+  rw [combinTheory.APPLY_UPDATE_THM,c_sem] >>
+  `SVARIANT (fv_P_c (csubst_P qc⦇s ↦ c_var s⦈ P)) NOTIN fv_P_c (csubst_P qc⦇s ↦ c_var s⦈ P)`
+    by METIS_TAC [SVARIANT_fv_P_c] >>
+  irule fv_c_eq_c_sem >>
+  rw [] >>
+  fs [combinTheory.APPLY_UPDATE_THM] >> rw [] >>
+  `SVARIANT (fv_P_c (csubst_P qc⦇s ↦ c_var s⦈ P)) IN
+   fv_P_c (csubst_P qc⦇s ↦ c_var s⦈ P)` suffices_by METIS_TAC [] >>
+  `fv_c (qc q) SUBSET fv_P_c (csubst_P qc⦇s ↦ c_var s⦈ P)`
+    suffices_by METIS_TAC [SUBSET_DEF] >>
+  rw [SUBSET_DEF] >>
+  rw [csubst_P_fv_P_c] >>
+  Q.EXISTS_TAC `q` >>
+  rw [combinTheory.APPLY_UPDATE_THM],
+
+  fs [combinTheory.APPLY_UPDATE_THM] >>
+  EQ_TAC >> rw [] >-
+   (Q.EXISTS_TAC `qs` >> rw [] >>
+    `!q. q IN fv_P_c P ==> (c_sem Mc Mq⦇s ↦ qs⦈ ∘ qc⦇s ↦ c_var s⦈) q = ((c_sem Mc Mq ∘ qc)⦇s ↦ qs⦈) q`
+    suffices_by METIS_TAC [fv_P_c_eq_P_sem] >>
+    rw [] >>
+    Q.PAT_X_ASSUM `!y. Q` (STRIP_ASSUME_TAC o (Q.SPECL [`q`])) >-
+     (rw [combinTheory.APPLY_UPDATE_THM,c_sem]) >>
+    Cases_on `s = q` >> fs [combinTheory.APPLY_UPDATE_THM,fv_c] >>
+    METIS_TAC [fv_c_notin_c_sem]) >>
+  Q.EXISTS_TAC `qs` >> rw [] >>
+  `!q. q IN fv_P_c P ==> (c_sem Mc Mq⦇s ↦ qs⦈ ∘ qc⦇s ↦ c_var s⦈) q = ((c_sem Mc Mq ∘ qc)⦇s ↦ qs⦈) q`
+    suffices_by METIS_TAC [fv_P_c_eq_P_sem] >>
+  rw [] >>
+  Q.PAT_X_ASSUM `!y. Q` (STRIP_ASSUME_TAC o (Q.SPECL [`q`])) >-
+   (rw [combinTheory.APPLY_UPDATE_THM,c_sem]) >>
+  Cases_on `s = q` >> fs [combinTheory.APPLY_UPDATE_THM,fv_c] >>
+  METIS_TAC [fv_c_notin_c_sem],
+
+  rw [c_sem_csubst]
+ ]
+QED
+
+Theorem P_sem_Ssubst:
+ !P omega Mc MS Mq MV VS.
+  P_sem omega Mc MS Mq MV (Ssubst_P VS P) <=>
+  P_sem omega Mc MS Mq (S_sem omega MS MV o VS) P
+Proof
+ Induct_on `P` >> rw [P_sem,Ssubst_P,fv_P_S,fv_S] >| [
+  rw [S_sem_Ssubst],
+
+  rw [S_sem_Ssubst],
+
+  rw [S_sem_Ssubst],
+
+  fs [combinTheory.APPLY_UPDATE_THM] >>
+  Cases_on `s = y` >> fs [fv_S] >>
+  EQ_TAC >> rw [] >-
+   (`!V. V IN fv_P_S P ==> 
+    (S_sem omega MS MV⦇SVARIANT (fv_P_S (Ssubst_P VS⦇s ↦ S_var s⦈ P)) ↦ Vs⦈ o
+      VS⦇s ↦ S_var (SVARIANT (fv_P_S (Ssubst_P VS⦇s ↦ S_var s⦈ P)))⦈) V =
+    ((S_sem omega MS MV o VS)⦇s ↦ Vs⦈) V`
+     suffices_by METIS_TAC [fv_P_S_eq_P_sem] >>
+
+    rw [combinTheory.APPLY_UPDATE_THM,S_sem] >>
+    `SVARIANT (fv_P_S (Ssubst_P VS⦇s ↦ S_var s⦈ P)) NOTIN fv_P_S (Ssubst_P VS⦇s ↦ S_var s⦈ P)`
+     by METIS_TAC [SVARIANT_fv_P_S] >>
+    irule fv_S_eq_S_sem >>
+    rw [] >>
+    fs [combinTheory.APPLY_UPDATE_THM] >> rw [] >>
+    `SVARIANT (fv_P_S (Ssubst_P VS⦇s ↦ S_var s⦈ P)) IN
+     fv_P_S (Ssubst_P VS⦇s ↦ S_var s⦈ P)` suffices_by METIS_TAC [] >>
+    `fv_S (VS V) SUBSET fv_P_S (Ssubst_P VS⦇s ↦ S_var s⦈ P)`
+     suffices_by METIS_TAC [SUBSET_DEF] >>
+    rw [SUBSET_DEF] >>
+    rw [Ssubst_P_fv_P_S] >>
+    Q.EXISTS_TAC `V` >>
+    rw [combinTheory.APPLY_UPDATE_THM]) >>
+  `!V. V IN fv_P_S P ==> 
+   (S_sem omega MS MV⦇SVARIANT (fv_P_S (Ssubst_P VS⦇s ↦ S_var s⦈ P)) ↦ Vs⦈ o
+     VS⦇s ↦ S_var (SVARIANT (fv_P_S (Ssubst_P VS⦇s ↦ S_var s⦈ P)))⦈) V =
+  ((S_sem omega MS MV o VS)⦇s ↦ Vs⦈) V`
+    suffices_by METIS_TAC [fv_P_S_eq_P_sem] >>
+  rw [combinTheory.APPLY_UPDATE_THM,S_sem] >>
+  `SVARIANT (fv_P_S (Ssubst_P VS⦇s ↦ S_var s⦈ P)) NOTIN fv_P_S (Ssubst_P VS⦇s ↦ S_var s⦈ P)`
+    by METIS_TAC [SVARIANT_fv_P_S] >>
+  irule fv_S_eq_S_sem >>
+  rw [] >>
+  fs [combinTheory.APPLY_UPDATE_THM] >> rw [] >>
+  `SVARIANT (fv_P_S (Ssubst_P VS⦇s ↦ S_var s⦈ P)) IN
+   fv_P_S (Ssubst_P VS⦇s ↦ S_var s⦈ P)` suffices_by METIS_TAC [] >>
+  `fv_S (VS V) SUBSET fv_P_S (Ssubst_P VS⦇s ↦ S_var s⦈ P)`
+    suffices_by METIS_TAC [SUBSET_DEF] >>
+  rw [SUBSET_DEF] >>
+  rw [Ssubst_P_fv_P_S] >>
+  Q.EXISTS_TAC `V` >>
+  rw [combinTheory.APPLY_UPDATE_THM],
+
+  fs [combinTheory.APPLY_UPDATE_THM] >>
+  EQ_TAC >> rw [] >-
+   (`!V. V IN fv_P_S P ==>
+     (S_sem omega MS MV⦇s ↦ Vs⦈ o VS⦇s ↦ S_var s⦈) V =
+     ((S_sem omega MS MV o VS)⦇s ↦ Vs⦈) V`
+    suffices_by METIS_TAC [fv_P_S_eq_P_sem] >>
+    rw [] >>
+    Q.PAT_X_ASSUM `!y. Q \/ R` (STRIP_ASSUME_TAC o (Q.SPECL [`V`])) >-
+     (rw [combinTheory.APPLY_UPDATE_THM,S_sem]) >>
+    Cases_on `s = V` >> fs [combinTheory.APPLY_UPDATE_THM,fv_S] >>
+    METIS_TAC [fv_S_notin_S_sem]) >>
+  `!V. V IN fv_P_S P ==>
+    (S_sem omega MS MV⦇s ↦ Vs⦈ ∘ VS⦇s ↦ S_var s⦈) V = ((S_sem omega MS MV o VS)⦇s ↦ Vs⦈) V`
+    suffices_by METIS_TAC [fv_P_S_eq_P_sem] >>
+  rw [] >>
+  Q.PAT_X_ASSUM `!y. Q \/ R` (STRIP_ASSUME_TAC o (Q.SPECL [`V`])) >-
+   (rw [combinTheory.APPLY_UPDATE_THM,S_sem]) >>
+  Cases_on `s = V` >> fs [combinTheory.APPLY_UPDATE_THM,fv_S] >>
+  METIS_TAC [fv_S_notin_S_sem],
+
+  fs [combinTheory.APPLY_UPDATE_THM] >>
+  Cases_on `s = y` >> fs [fv_S] >>
+  EQ_TAC >> rw [] >-
+   (`!V. V IN fv_P_S P ==> 
+    (S_sem omega MS MV⦇SVARIANT (fv_P_S (Ssubst_P VS⦇s ↦ S_var s⦈ P)) ↦ Vs⦈ o
+      VS⦇s ↦ S_var (SVARIANT (fv_P_S (Ssubst_P VS⦇s ↦ S_var s⦈ P)))⦈) V =
+    ((S_sem omega MS MV o VS)⦇s ↦ Vs⦈) V`
+     suffices_by METIS_TAC [fv_P_S_eq_P_sem] >>
+
+    rw [combinTheory.APPLY_UPDATE_THM,S_sem] >>
+    `SVARIANT (fv_P_S (Ssubst_P VS⦇s ↦ S_var s⦈ P)) NOTIN fv_P_S (Ssubst_P VS⦇s ↦ S_var s⦈ P)`
+     by METIS_TAC [SVARIANT_fv_P_S] >>
+    irule fv_S_eq_S_sem >>
+    rw [] >>
+    fs [combinTheory.APPLY_UPDATE_THM] >> rw [] >>
+    `SVARIANT (fv_P_S (Ssubst_P VS⦇s ↦ S_var s⦈ P)) IN
+     fv_P_S (Ssubst_P VS⦇s ↦ S_var s⦈ P)` suffices_by METIS_TAC [] >>
+    `fv_S (VS V) SUBSET fv_P_S (Ssubst_P VS⦇s ↦ S_var s⦈ P)`
+     suffices_by METIS_TAC [SUBSET_DEF] >>
+    rw [SUBSET_DEF] >>
+    rw [Ssubst_P_fv_P_S] >>
+    Q.EXISTS_TAC `V` >>
+    rw [combinTheory.APPLY_UPDATE_THM]) >>
+  `!V. V IN fv_P_S P ==> 
+   (S_sem omega MS MV⦇SVARIANT (fv_P_S (Ssubst_P VS⦇s ↦ S_var s⦈ P)) ↦ Vs⦈ o
+     VS⦇s ↦ S_var (SVARIANT (fv_P_S (Ssubst_P VS⦇s ↦ S_var s⦈ P)))⦈) V =
+  ((S_sem omega MS MV o VS)⦇s ↦ Vs⦈) V`
+    suffices_by METIS_TAC [fv_P_S_eq_P_sem] >>
+  rw [combinTheory.APPLY_UPDATE_THM,S_sem] >>
+  `SVARIANT (fv_P_S (Ssubst_P VS⦇s ↦ S_var s⦈ P)) NOTIN fv_P_S (Ssubst_P VS⦇s ↦ S_var s⦈ P)`
+    by METIS_TAC [SVARIANT_fv_P_S] >>
+  irule fv_S_eq_S_sem >>
+  rw [] >>
+  fs [combinTheory.APPLY_UPDATE_THM] >> rw [] >>
+  `SVARIANT (fv_P_S (Ssubst_P VS⦇s ↦ S_var s⦈ P)) IN
+   fv_P_S (Ssubst_P VS⦇s ↦ S_var s⦈ P)` suffices_by METIS_TAC [] >>
+  `fv_S (VS V) SUBSET fv_P_S (Ssubst_P VS⦇s ↦ S_var s⦈ P)`
+    suffices_by METIS_TAC [SUBSET_DEF] >>
+  rw [SUBSET_DEF] >>
+  rw [Ssubst_P_fv_P_S] >>
+  Q.EXISTS_TAC `V` >>
+  rw [combinTheory.APPLY_UPDATE_THM],
+
+  fs [combinTheory.APPLY_UPDATE_THM] >>
+  EQ_TAC >> rw [] >-
+   (`!V. V IN fv_P_S P ==>
+     (S_sem omega MS MV⦇s ↦ Vs⦈ o VS⦇s ↦ S_var s⦈) V =
+     ((S_sem omega MS MV o VS)⦇s ↦ Vs⦈) V`
+    suffices_by METIS_TAC [fv_P_S_eq_P_sem] >>
+    rw [] >>
+    Q.PAT_X_ASSUM `!y. Q \/ R` (STRIP_ASSUME_TAC o (Q.SPECL [`V`])) >-
+     (rw [combinTheory.APPLY_UPDATE_THM,S_sem]) >>
+    Cases_on `s = V` >> fs [combinTheory.APPLY_UPDATE_THM,fv_S] >>
+    METIS_TAC [fv_S_notin_S_sem]) >>
+  `!V. V IN fv_P_S P ==>
+    (S_sem omega MS MV⦇s ↦ Vs⦈ ∘ VS⦇s ↦ S_var s⦈) V = ((S_sem omega MS MV o VS)⦇s ↦ Vs⦈) V`
+    suffices_by METIS_TAC [fv_P_S_eq_P_sem] >>
+  rw [] >>
+  Q.PAT_X_ASSUM `!y. Q \/ R` (STRIP_ASSUME_TAC o (Q.SPECL [`V`])) >-
+   (rw [combinTheory.APPLY_UPDATE_THM,S_sem]) >>
+  Cases_on `s = V` >> fs [combinTheory.APPLY_UPDATE_THM,fv_S] >>
+  METIS_TAC [fv_S_notin_S_sem],
+
+  rw [S_sem_Ssubst]
+ ]
+QED
+
+Theorem P_sem_csubst1:
+ !P omega Mc MS Mq MV c q.
+  P_sem omega Mc MS Mq MV (csubst_P ((q =+ c) c_var) P) <=>
+  P_sem omega Mc MS ((q =+ c_sem Mc Mq c) Mq) MV P
+Proof
+ simp[P_sem_csubst] >> 
+ rw [] >>
+ irule fv_P_c_eq_P_sem >>
+ rw[combinTheory.APPLY_UPDATE_THM,c_sem]
+QED
+
+Theorem P_sem_Ssubst1:
+ !P omega Mc MS Mq MV S V.
+  P_sem omega Mc MS Mq MV (Ssubst_P ((V =+ S) S_var) P) <=>
+  P_sem omega Mc MS Mq ((V =+ S_sem omega MS MV S) MV) P
+Proof
+ simp[P_sem_Ssubst] >> 
+ rw [] >>
+ irule fv_P_S_eq_P_sem >>
+ rw[combinTheory.APPLY_UPDATE_THM,S_sem]
+QED
+
+Theorem P_sem_rename_c:
+ !P omega Mc MS Mq MV x y.
+  P_sem omega Mc MS Mq MV (csubst_P ((x =+ c_var y) c_var) P) <=>
+  P_sem omega Mc MS ((x =+ Mq y) Mq) MV P
+Proof
+ rw [P_sem_csubst1,c_sem]
+QED
+
+Theorem P_sem_rename_S:
+ !P omega Mc MS Mq MV x y.
+  P_sem omega Mc MS Mq MV (Ssubst_P ((x =+ S_var y) S_var) P) <=>
+  P_sem omega Mc MS Mq ((x =+ MV y) MV) P
+Proof
+ rw [P_sem_Ssubst1,S_sem]
+QED
+
+Theorem P_sem_alpha_forall_c:
+ !P omega Mc MS Mq MV x y. y NOTIN fv_P_c (P_forall_c x P) ==>
+ (P_sem omega Mc MS Mq MV (P_forall_c y (csubst_P ((x =+ c_var y) c_var) P)) <=>
+  P_sem omega Mc MS Mq MV (P_forall_c x P))
+Proof
+ rw [P_sem,P_sem_csubst1,c_sem,fv_P_c] >> 
+ EQ_TAC >> rw [] >-
+  (`P_sem omega Mc MS ((x =+ qs) ((y =+ qs) Mq)) MV P`
+    by METIS_TAC [] >>
+   `(!q. q IN fv_P_c P ==> ((x =+ qs) ((y =+ qs) Mq)) q = ((x =+ qs) Mq) q)`
+    suffices_by METIS_TAC [fv_P_c_eq_P_sem] >>
+   rw [] >>
+   `q <> y` by METIS_TAC [] >>
+   rw [combinTheory.APPLY_UPDATE_THM]) >>
+ `P_sem omega Mc MS ((x =+ qs) Mq) MV P`
+  by METIS_TAC [] >>
+ `(!q. q IN fv_P_c P ==> ((x =+ qs) ((y =+ qs) Mq)) q = ((x =+ qs) Mq) q)`
+  suffices_by METIS_TAC [fv_P_c_eq_P_sem] >>
+ rw [] >>
+ `q <> y` by METIS_TAC [] >>
+ rw [combinTheory.APPLY_UPDATE_THM]
+QED
+
+Theorem P_sem_alpha_forall_S:
+ !P omega Mc MS Mq MV x y. y NOTIN fv_P_S (P_forall_S x P) ==>
+ (P_sem omega Mc MS Mq MV (P_forall_S y (Ssubst_P ((x =+ S_var y) S_var) P)) <=>
+  P_sem omega Mc MS Mq MV (P_forall_S x P))
+Proof
+ rw [P_sem,P_sem_Ssubst1,S_sem,fv_P_S] >> 
+ EQ_TAC >> rw [] >-
+  (`P_sem omega Mc MS Mq ((x =+ Vs) ((y =+ Vs) MV)) P`
+    by METIS_TAC [] >>
+   `(!V. V IN fv_P_S P ==> ((x =+ Vs) ((y =+ Vs) MV)) V = ((x =+ Vs) MV) V)`
+    suffices_by METIS_TAC [fv_P_S_eq_P_sem] >>
+   rw [] >>
+   `V <> y` by METIS_TAC [] >>
+   rw [combinTheory.APPLY_UPDATE_THM]) >>
+ `P_sem omega Mc MS Mq ((x =+ Vs) MV) P`
+  by METIS_TAC [] >>
+ `(!V. V IN fv_P_S P ==> ((x =+ Vs) ((y =+ Vs) MV)) V = ((x =+ Vs) MV) V)`
+  suffices_by METIS_TAC [fv_P_S_eq_P_sem] >>
+ rw [] >>
+ `V <> y` by METIS_TAC [] >>
+ rw [combinTheory.APPLY_UPDATE_THM]
+QED
+
+(* proof system soundness *)
+
+Theorem spec_holds_system_sound:
+ !omega. spec_system_sound spec_holds omega
+Proof
+ strip_tac >>
+ `!G P. spec_holds G P ==>
+  !Mc Mq MS MV.
+  (!s. Mc s SUBSET omega) /\
+  (!s. Mq s SUBSET omega) /\
+  (!s. MS s SUBSET POW omega) /\
+  (!s. MV s SUBSET POW omega) /\
+   (!P0. P0 IN G ==> P_sem omega Mc MS Mq MV P0) ==> P_sem omega Mc MS Mq MV P`
   suffices_by METIS_TAC [spec_system_sound] >>
- ho_match_mp_tac spec_holds_ind >> rw [] >| [
+ ho_match_mp_tac spec_proof_ind >> rw [] >| [
+  (* ri *)
+  fs [P_sem] >> fs [c_sem] >>
+  rw [SUBSET_DEF] >>
+  fs [APPLY_UPDATE_THM] >>
+  `S_sem omega MS MV S1 SUBSET POW omega`
+   by METIS_TAC [S_sem_omega] >>
+  qsuff_tac `x SUBSET omega` >- METIS_TAC [] >>
+  fs [POW_DEF,SUBSET_DEF] >> METIS_TAC [],
+
   (* re *)
   METIS_TAC [proposition_2a],
 
-  (* am *)
-  METIS_TAC [proposition3_b],
+  (* am1 *)
+  METIS_TAC [proposition_3a],
+
+  (* am2 *)
+  METIS_TAC [proposition_3b],
 
   (* conji *)
   METIS_TAC [proposition_4a],
@@ -503,49 +1599,436 @@ Proof
   (* conje2 *)
   METIS_TAC [proposition_4b_alt],
 
-  (* ce *)
-  METIS_TAC [proposition_7a_alt],
+  (* pi *)
+  rw [P_sem] >> rw [c_sem] >> rw [S_sem] >>
+  rw [double_intersection] >>
+  Q.EXISTS_TAC `c_sem Mc Mq c1` >>
+  Q.EXISTS_TAC `c_sem Mc Mq c2` >>
+  fs [P_sem],
+
+  (* pe *)
+  METIS_TAC [proposition_5a],
 
   (* ci *)
   METIS_TAC [proposition_7b],
 
+  (* ce *)
+  METIS_TAC [proposition_7a_alt],
+
   (* cre *)
-  METIS_TAC [proposition_4b_alt,proposition_2a,proposition_4a]
+  `P_sem omega Mc MS Mq MV (P_implements c (S_conj S1 S2))` by METIS_TAC [] >>
+  METIS_TAC [proposition_4b_alt,proposition_2a,proposition_4a],
+
+  (* cr *)
+  `P_sem omega Mc MS Mq MV (P_implements c (S_conj S1 S3))` by METIS_TAC [] >>
+  `P_sem omega Mc MS Mq MV (P_refines S1 S2)` by METIS_TAC [] >>
+  fs [P_sem,S_sem] >>
+  METIS_TAC [SUBSET_DEF],
+
+  (* andi *)
+  rw [P_sem],
+
+  (* ande1 *)
+  `P_sem omega Mc MS Mq MV (P_and P P2)` by METIS_TAC [] >>
+  METIS_TAC [P_sem],
+
+  (* ande2 *)
+  `P_sem omega Mc MS Mq MV (P_and P1 P)` by METIS_TAC [] >>
+  METIS_TAC [P_sem],
+
+  (* impi *)
+  rw [P_sem] >>
+  `!P0. P0 = P1 \/ P0 IN G ==> P_sem omega Mc MS Mq MV P0`
+   by METIS_TAC [] >>
+  METIS_TAC [],
+
+  (* impe *)
+  `P_sem omega Mc MS Mq MV (P_implies P' P)` by METIS_TAC [] >>
+  `P_sem omega Mc MS Mq MV P'` by METIS_TAC [] >>
+  METIS_TAC [P_sem],
+
+  (* ori1 *)
+  `P_sem omega Mc MS Mq MV P`
+   by METIS_TAC [] >>
+  METIS_TAC [P_sem],
+
+  (* ori2 *)
+  `P_sem omega Mc MS Mq MV P`
+   by METIS_TAC [] >>
+  METIS_TAC [P_sem],
+
+  (* orel *)
+  `P_sem omega Mc MS Mq MV (P_or P1 P2)` by METIS_TAC [] >>
+  fs [P_sem] >-
+   (`!P0. P0 = P1 \/ P0 IN G ==> P_sem omega Mc MS Mq MV P0`
+     by METIS_TAC [] >>
+    METIS_TAC []) >>
+  `!P0. P0 = P2 \/ P0 IN G ==> P_sem omega Mc MS Mq MV P0`
+   by METIS_TAC [] >>
+  METIS_TAC [],
+
+  (* notin *)
+  rw [P_sem] >> strip_tac >>
+  `!P0. P0 = P1 \/ P0 IN G ==> P_sem omega Mc MS Mq MV P0`
+   by METIS_TAC [] >>
+  `P_sem omega Mc MS Mq MV P` by METIS_TAC [] >>
+  `P_sem omega Mc MS Mq MV (P_not P)` by METIS_TAC [] >>
+  METIS_TAC [P_sem],
+
+  (* notel *)
+  `P_sem omega Mc MS Mq MV (P_not (P_not P))`
+   by METIS_TAC [] >>
+  METIS_TAC [P_sem],
+
+  (* allel *)
+  `P_sem omega Mc MS Mq MV (P_forall_c q P)` by METIS_TAC [] >>
+  fs [P_sem] >>
+  `c_sem Mc Mq c SUBSET omega` by METIS_TAC [c_sem_omega] >>
+  `P_sem omega Mc MS ((q =+ c_sem Mc Mq c) Mq) MV P` by METIS_TAC [] >>
+  METIS_TAC [P_sem_csubst1],
+
+  (* allin *)
+  rw [P_sem] >>
+  `!s. ((q' =+ qs) Mq) s SUBSET omega`
+   by rw [APPLY_UPDATE_THM] >>
+  sg `!P0. P0 IN G ==> P_sem omega Mc MS ((q' =+ qs) Mq) MV P0` >-
+   (rw [] >>
+    `q' NOTIN fv_P_c P0` by METIS_TAC [] >>
+    `P_sem omega Mc MS Mq MV P0` by METIS_TAC [] >>
+    `!q0. q0 IN fv_P_c P0 ==> ((q' =+ qs) Mq) q0 = Mq q0`
+    suffices_by METIS_TAC [fv_P_c_eq_P_sem] >>
+    rw [APPLY_UPDATE_THM] >> METIS_TAC []) >>
+  `P_sem omega Mc MS ((q' =+ qs) Mq) MV (csubst_P c_var⦇q ↦ c_var q'⦈ P)`
+   by METIS_TAC [] >>
+  `P_sem omega Mc MS ((q =+ (Mq⦇q' ↦ qs⦈) q') (Mq⦇q' ↦ qs⦈)) MV P`
+   by METIS_TAC [P_sem_rename_c] >>
+  fs [APPLY_UPDATE_THM] >>
+  `!q0. q0 IN fv_P_c P ==> (Mq⦇q ↦ qs; q' ↦ qs⦈) q0 = (Mq⦇q ↦ qs⦈) q0`
+   suffices_by METIS_TAC [fv_P_c_eq_P_sem] >>
+  rw [APPLY_UPDATE_THM] >> METIS_TAC [],
+
+  (* eq_el_c *)
+  `P_sem omega Mc MS Mq MV (P_c_eq c c')` by METIS_TAC [] >>
+  `P_sem omega Mc MS Mq MV (csubst_P c_var⦇q ↦ c⦈ P)` by METIS_TAC [] >>  
+  fs [P_sem_csubst1,P_sem] >>
+  METIS_TAC [],
+
+  (* all_el_S *)
+  `P_sem omega Mc MS Mq MV (P_forall_S V P)` by METIS_TAC [] >>
+  fs [P_sem] >>
+  `S_sem omega MS MV S' SUBSET POW omega` by METIS_TAC [S_sem_omega] >>
+  `P_sem omega Mc MS Mq ((V =+ S_sem omega MS MV S') MV) P` by METIS_TAC [] >>
+  METIS_TAC [P_sem_Ssubst1],
+
+  (* all_in_S *)
+  rw [P_sem] >>
+  `!s. ((V' =+ Vs) MV) s SUBSET POW omega`
+   by rw [APPLY_UPDATE_THM] >>
+  sg `!P0. P0 IN G ==> P_sem omega Mc MS Mq ((V' =+ Vs) MV) P0` >-
+   (rw [] >>
+    `V' NOTIN fv_P_S P0` by METIS_TAC [] >>
+    `P_sem omega Mc MS Mq MV P0` by METIS_TAC [] >>
+    `!V0. V0 IN fv_P_S P0 ==> ((V' =+ Vs) MV) V0 = MV V0`
+    suffices_by METIS_TAC [fv_P_S_eq_P_sem] >>
+    rw [APPLY_UPDATE_THM] >> METIS_TAC []) >>
+  `P_sem omega Mc MS Mq ((V' =+ Vs) MV) (Ssubst_P S_var⦇V ↦ S_var V'⦈ P)`
+   by METIS_TAC [] >>
+  `P_sem omega Mc MS Mq ((V =+ (MV⦇V' ↦ Vs⦈) V') (MV⦇V' ↦ Vs⦈)) P`
+   by METIS_TAC [P_sem_rename_S] >>
+  fs [APPLY_UPDATE_THM] >>
+  `!V0. V0 IN fv_P_S P ==> (MV⦇V ↦ Vs; V' ↦ Vs⦈) V0 = (MV⦇V ↦ Vs⦈) V0`
+   suffices_by METIS_TAC [fv_P_S_eq_P_sem] >>
+  rw [APPLY_UPDATE_THM] >> METIS_TAC [],
+
+  (* eq_el_S *)
+  `P_sem omega Mc MS Mq MV (P_S_eq S'' S')` by METIS_TAC [] >>
+  `P_sem omega Mc MS Mq MV (Ssubst_P S_var⦇V ↦ S''⦈ P)` by METIS_TAC [] >>  
+  fs [P_sem_Ssubst1,P_sem] >>
+  METIS_TAC [],
+
+  (* ex_in_c *)
+  `P_sem omega Mc MS Mq MV (csubst_P ((q =+ c) c_var) P)`
+   by METIS_TAC [] >>
+  rw [P_sem] >>
+  Q.EXISTS_TAC `c_sem Mc Mq c` >>
+  rw [] >- METIS_TAC [c_sem_omega] >>
+  METIS_TAC [P_sem_csubst1],
+
+  (* ex_el_c *)
+  fs [P_sem] >>
+  sg `!qs P0. P0 IN G ==> P_sem omega Mc MS ((q' =+ qs) Mq) MV P0` >-
+   (rw [] >>
+    `q' NOTIN fv_P_c P0` by METIS_TAC [] >>
+    `P_sem omega Mc MS Mq MV P0` by METIS_TAC [] >>
+    `!q0. q0 IN fv_P_c P0 ==> ((q' =+ qs) Mq) q0 = Mq q0`
+    suffices_by METIS_TAC [fv_P_c_eq_P_sem] >>
+    rw [APPLY_UPDATE_THM] >> METIS_TAC []) >>
+  `?qs. qs SUBSET omega /\ P_sem omega Mc MS ((q =+ qs) Mq) MV P'` by METIS_TAC [] >>
+  sg `P_sem omega Mc MS ((q =+ (Mq⦇q' ↦ qs⦈) q') (Mq⦇q' ↦ qs⦈)) MV P'` >-
+   (rw [P_sem_csubst1] >>
+    `!q0. q0 IN fv_P_c P' ==> (Mq⦇q ↦ qs; q' ↦ qs⦈) q0 = (Mq⦇q ↦ qs⦈) q0`
+     suffices_by METIS_TAC [fv_P_c_eq_P_sem] >>
+    rw [APPLY_UPDATE_THM] >> METIS_TAC []) >>      
+  `P_sem omega Mc MS (Mq⦇q' ↦ qs⦈) MV (csubst_P c_var⦇q ↦ c_var q'⦈ P')`
+   by METIS_TAC [P_sem_rename_c] >>
+  sg `!P0. P0 IN G' ==> P_sem omega Mc MS Mq⦇q' ↦ qs⦈ MV P0` >-
+   (rw [] >>
+    `P_sem omega Mc MS Mq MV P0` by METIS_TAC [] >>
+    `!q0. q0 IN fv_P_c P0 ==> (Mq⦇q' ↦ qs⦈) q0 = Mq q0`
+     suffices_by METIS_TAC [fv_P_c_eq_P_sem] >>
+    rw [APPLY_UPDATE_THM] >> METIS_TAC []) >>
+  `!s. (Mq⦇q' ↦ qs⦈) s SUBSET omega` by rw [APPLY_UPDATE_THM] >>
+  `P_sem omega Mc MS Mq⦇q' ↦ qs⦈ MV P` by METIS_TAC [] >>
+  `!q0. q0 IN fv_P_c P ==> (Mq⦇q' ↦ qs⦈) q0 = Mq q0`
+   suffices_by METIS_TAC [fv_P_c_eq_P_sem] >>
+  rw [APPLY_UPDATE_THM] >> METIS_TAC [],
+
+  (* ex_in_S *)
+  `P_sem omega Mc MS Mq MV (Ssubst_P ((V =+ S') S_var) P)`
+   by METIS_TAC [] >>
+  rw [P_sem] >>
+  Q.EXISTS_TAC `S_sem omega MS MV S'` >>
+  rw [] >- METIS_TAC [S_sem_omega] >>
+  METIS_TAC [P_sem_Ssubst1],
+
+  (* ex_el_S *)
+  fs [P_sem] >>
+  sg `!VS P0. P0 IN G ==> P_sem omega Mc MS Mq ((V' =+ VS) MV) P0` >-
+   (rw [] >>
+    `V' NOTIN fv_P_S P0` by METIS_TAC [] >>
+    `P_sem omega Mc MS Mq MV P0` by METIS_TAC [] >>
+    `!V0. V0 IN fv_P_S P0 ==> ((V' =+ VS) MV) V0 = MV V0`
+     suffices_by METIS_TAC [fv_P_S_eq_P_sem] >>
+    rw [APPLY_UPDATE_THM] >> METIS_TAC []) >>
+  `?VS. VS SUBSET POW omega /\ P_sem omega Mc MS Mq ((V =+ VS) MV) P'` by METIS_TAC [] >>
+  sg `P_sem omega Mc MS Mq ((V =+ (MV⦇V' ↦ VS⦈) V') (MV⦇V' ↦ VS⦈)) P'` >-
+   (rw [P_sem_Ssubst1] >>
+    `!V0. V0 IN fv_P_S P' ==> (MV⦇V ↦ VS; V' ↦ VS⦈) V0 = (MV⦇V ↦ VS⦈) V0`
+     suffices_by METIS_TAC [fv_P_S_eq_P_sem] >>
+    rw [APPLY_UPDATE_THM] >> METIS_TAC []) >>
+  `P_sem omega Mc MS Mq (MV⦇V' ↦ VS⦈) (Ssubst_P S_var⦇V ↦ S_var V'⦈ P')`
+   by METIS_TAC [P_sem_rename_S] >>
+  sg `!P0. P0 IN G' ==> P_sem omega Mc MS Mq MV⦇V' ↦ VS⦈ P0` >-
+   (rw [] >>
+    `P_sem omega Mc MS Mq MV P0` by METIS_TAC [] >>
+    `!V0. V0 IN fv_P_S P0 ==> (MV⦇V' ↦ VS⦈) V0 = MV V0`
+     suffices_by METIS_TAC [fv_P_S_eq_P_sem] >>
+    rw [APPLY_UPDATE_THM] >> METIS_TAC []) >>
+
+  `!s. (MV⦇V' ↦ VS⦈) s SUBSET POW omega` by rw [APPLY_UPDATE_THM] >>
+  `P_sem omega Mc MS Mq MV⦇V' ↦ VS⦈ P` by METIS_TAC [] >>
+  `!V0. V0 IN fv_P_S P ==> (MV⦇V' ↦ VS⦈) V0 = MV V0`
+   suffices_by METIS_TAC [fv_P_S_eq_P_sem] >>
+  rw [APPLY_UPDATE_THM] >> METIS_TAC []
  ]
 QED
 
-Theorem contract_compositionality_sem_two:
- !Mc MS Mq MV S1 S2 A1 A2 G1 G2 q1 q2.
+(* proving compositionality *)
+
+Theorem implements_comp_refines_two:
+ !omega Mc MS Mq MV S0 S1 S2 q1 q2.
+  (!s. MS s SUBSET POW omega) /\
+  (!s. MV s SUBSET POW omega) /\
   q1 <> q2 /\
-  (P_sem Mc MS Mq MV
+  (P_sem omega Mc MS Mq MV
+  (P_forall_c q1 (P_forall_c q2
+   (P_implies
+     (P_and (P_implements (c_var q1) S1) (P_implements (c_var q2) S2))
+     (P_implements (c_comp (c_var q1) (c_var q2)) S0))))) ==>
+  P_sem omega Mc MS Mq MV (P_refines (S_par S1 S2) S0)
+Proof
+ rw [P_sem,c_sem,S_sem,APPLY_UPDATE_THM] >>
+ Cases_on `q2 = q1` >> fs [] >>
+ rw [double_intersection,SUBSET_DEF] >>
+ METIS_TAC [IN_POW,SUBSET_DEF,S_sem_omega]
+QED
+
+Theorem contract_compositionality_sem_two:
+ !omega Mc MS Mq MV A G A1 A2 G1 G2 q1 q2.
+  (!s. MS s SUBSET POW omega) /\
+  (!s. MV s SUBSET POW omega) /\
+  q1 <> q2 /\
+  (P_sem omega Mc MS Mq MV
   (P_forall_c q1 (P_forall_c q2
    (P_implies
      (P_and (P_implements (c_var q1) (S_assume A1 G1)) (P_implements (c_var q2) (S_assume A2 G2)))
-     (P_implements (c_comp (c_var q1) (c_var q2)) (S_assume S1 S2)))))) ==>
-  P_sem Mc MS Mq MV (P_refines (S_par (S_assume A1 G1) (S_assume A2 G2)) (S_assume S1 S2))
+     (P_implements (c_comp (c_var q1) (c_var q2)) (S_assume A G)))))) ==>
+  P_sem omega Mc MS Mq MV (P_refines (S_par (S_assume A1 G1) (S_assume A2 G2)) (S_assume A G))
 Proof
- rw [P_sem,c_sem,APPLY_UPDATE_THM] >>
- rw [SUBSET_DEF] >>
- `?a b. x = a INTER b /\ a IN S_sem MS MV (S_assume A1 G1) /\ b IN S_sem MS MV (S_assume A2 G2)`
-  by METIS_TAC [S_sem_IN_par_IN] >>
- rw [] >> Cases_on `q1 = q2` >> fs []
+ METIS_TAC [implements_comp_refines_two]
 QED
 
 Theorem contract_compositionality_system_two:
- !R Mc MS Mq MV.
- spec_system_sound R Mc MS Mq MV ==>
- !G. (!P0. P0 IN G ==> P_sem Mc MS Mq MV P0) ==>
- !S1 S2 A1 A2 G1 G2 q1 q2.
-  q1 <> q2 ==>
-  R G (P_forall_c q1 (P_forall_c q2 (P_implies
+ !R omega Mc MS Mq MV.
+ spec_system_sound R omega /\
+ (!s. Mc s SUBSET omega) /\
+ (!s. Mq s SUBSET omega) /\
+ (!s. MS s SUBSET POW omega) /\
+ (!s. MV s SUBSET POW omega) ==>
+ !Gamma. (!P0. P0 IN Gamma ==> P_sem omega Mc MS Mq MV P0) ==>
+ !A G A1 A2 G1 G2 q1 q2.
+  q1 <> q2 /\
+  R Gamma (P_forall_c q1 (P_forall_c q2 (P_implies
    (P_and (P_implements (c_var q1) (S_assume A1 G1)) (P_implements (c_var q2) (S_assume A2 G2)))
-   (P_implements (c_comp (c_var q1) (c_var q2)) (S_assume S1 S2))))) ==>
- P_sem Mc MS Mq MV (P_refines (S_par (S_assume A1 G1) (S_assume A2 G2)) (S_assume S1 S2))
+   (P_implements (c_comp (c_var q1) (c_var q2)) (S_assume A G))))) ==>
+ P_sem omega Mc MS Mq MV (P_refines (S_par (S_assume A1 G1) (S_assume A2 G2)) (S_assume A G))
 Proof
  rw [spec_system_sound] >>
  match_mp_tac contract_compositionality_sem_two >>
  Q.EXISTS_TAC `q1` >> Q.EXISTS_TAC `q2` >>
  rw [] >> METIS_TAC []
+QED
+
+Theorem implements_comp_refines_three:
+ !omega Mc MS Mq MV S0 S1 S2 S3 q1 q2 q3.
+  (!s. MS s SUBSET POW omega) /\
+  (!s. MV s SUBSET POW omega) /\
+  q1 <> q2 /\ q1 <> q3 /\ q2 <> q3 /\
+  (P_sem omega Mc MS Mq MV
+   (P_forall_c q1 (P_forall_c q2 (P_forall_c q3
+    (P_implies
+     (P_and (P_implements (c_var q1) S1) (P_and (P_implements (c_var q2) S2) (P_implements (c_var q3) S3)))
+     (P_implements (c_comp (c_var q1) (c_comp (c_var q2) (c_var q3))) S0)))))) ==>
+  P_sem omega Mc MS Mq MV (P_refines (S_par S1 (S_par S2 S3)) S0)
+Proof
+ rw [P_sem,c_sem,S_sem,APPLY_UPDATE_THM] >>
+ Cases_on `q2 = q1` >> fs [] >>
+ Cases_on `q3 = q1` >> fs [] >>
+ Cases_on `q3 = q2` >> fs [] >> 
+ rw [double_intersection,SUBSET_DEF] >>
+ METIS_TAC [IN_POW,SUBSET_DEF,S_sem_omega]
+QED
+
+Theorem contract_compositionality_sem_three:
+ !omega Mc MS Mq MV A G A1 G1 A2 G2 A3 G3 q1 q2 q3.
+  (!s. MS s SUBSET POW omega) /\
+  (!s. MV s SUBSET POW omega) /\
+  q1 <> q2 /\ q1 <> q3 /\ q2 <> q3 /\
+  (P_sem omega Mc MS Mq MV
+   (P_forall_c q1 (P_forall_c q2 (P_forall_c q3
+    (P_implies
+     (P_and (P_implements (c_var q1) (S_assume A1 G1))
+      (P_and (P_implements (c_var q2) (S_assume A2 G2)) (P_implements (c_var q3) (S_assume A3 G3))))
+     (P_implements (c_comp (c_var q1) (c_comp (c_var q2) (c_var q3))) (S_assume A G))))))) ==>
+  P_sem omega Mc MS Mq MV (P_refines (S_par (S_assume A1 G1) (S_par (S_assume A2 G2) (S_assume A3 G3))) (S_assume A G))
+Proof
+ METIS_TAC [implements_comp_refines_three]
+QED
+
+Theorem contract_compositionality_system_three:
+ !R omega Mc MS Mq MV.
+ spec_system_sound R omega /\
+ (!s. Mc s SUBSET omega) /\
+ (!s. Mq s SUBSET omega) /\
+ (!s. MS s SUBSET POW omega) /\
+ (!s. MV s SUBSET POW omega) ==>
+ !Gamma. (!P0. P0 IN Gamma ==> P_sem omega Mc MS Mq MV P0) ==>
+ !A G A1 G1 A2 G2 A3 G3 q1 q2 q3.
+  q1 <> q2 /\ q1 <> q3 /\ q2 <> q3 /\
+  R Gamma
+   (P_forall_c q1 (P_forall_c q2 (P_forall_c q3
+    (P_implies
+     (P_and (P_implements (c_var q1) (S_assume A1 G1))
+      (P_and (P_implements (c_var q2) (S_assume A2 G2)) (P_implements (c_var q3) (S_assume A3 G3))))
+     (P_implements (c_comp (c_var q1) (c_comp (c_var q2) (c_var q3))) (S_assume A G)))))) ==>   
+  P_sem omega Mc MS Mq MV (P_refines (S_par (S_assume A1 G1) (S_par (S_assume A2 G2) (S_assume A3 G3))) (S_assume A G))
+Proof
+ rw [spec_system_sound] >>
+ match_mp_tac contract_compositionality_sem_three >>
+ Q.EXISTS_TAC `q1` >> Q.EXISTS_TAC `q2` >> Q.EXISTS_TAC `q3` >>
+ rw [] >> METIS_TAC []
+QED
+
+Theorem implements_comp_three_refines:
+ !omega Mc MS Mq MV S0 S1 S2 S3 q1 q2 q3.
+  (!s. MS s SUBSET POW omega) /\
+  (!s. MV s SUBSET POW omega) /\
+  q1 <> q2 /\ q1 <> q3 /\ q2 <> q3 /\
+  P_sem omega Mc MS Mq MV (P_refines (S_par S1 (S_par S2 S3)) S0) ==>
+  (P_sem omega Mc MS Mq MV
+   (P_forall_c q1 (P_forall_c q2 (P_forall_c q3
+    (P_implies
+     (P_and (P_implements (c_var q1) S1) (P_and (P_implements (c_var q2) S2) (P_implements (c_var q3) S3)))
+     (P_implements (c_comp (c_var q1) (c_comp (c_var q2) (c_var q3))) S0))))))
+Proof
+ rw [P_sem,c_sem,S_sem,APPLY_UPDATE_THM] >>
+ fs [double_intersection,SUBSET_DEF] >>
+ METIS_TAC []
+QED
+
+Theorem implements_comp_three_refines_term:
+ !omega Mc MS Mq MV S0 S1 S2 S3 c1 c2 c3.
+  (!s. MS s SUBSET POW omega) /\
+  (!s. MV s SUBSET POW omega) /\
+  P_sem omega Mc MS Mq MV (P_refines (S_par S1 (S_par S2 S3)) S0) /\
+  P_sem omega Mc MS Mq MV (P_implements c1 S1) /\
+  P_sem omega Mc MS Mq MV (P_implements c2 S2) /\
+  P_sem omega Mc MS Mq MV (P_implements c3 S3) ==>
+  P_sem omega Mc MS Mq MV (P_implements (c_comp c1 (c_comp c2 c3)) S0)
+Proof
+ rw [P_sem,c_sem,S_sem] >>
+ fs [double_intersection,SUBSET_DEF] >>
+ METIS_TAC []
+QED
+
+Theorem compositionality_contracts_three:
+ !R omega Mc MS Mq MV.
+ spec_system_sound R omega /\
+ (!s. Mc s SUBSET omega) /\
+ (!s. Mq s SUBSET omega) /\
+ (!s. MS s SUBSET POW omega) /\
+ (!s. MV s SUBSET POW omega) ==>
+ !Gamma. (!P0. P0 IN Gamma ==> P_sem omega Mc MS Mq MV P0) ==>
+ !S0 S1 S2 S3 c1 c2 c3.
+ P_sem omega Mc MS Mq MV (P_refines (S_par S1 (S_par S2 S3)) S0) /\
+ R Gamma (P_implements c1 S1) /\
+ R Gamma (P_implements c2 S2) /\
+ R Gamma (P_implements c3 S3) ==>
+ P_sem omega Mc MS Mq MV (P_implements (c_comp c1 (c_comp c2 c3)) S0)
+Proof
+ rw [spec_system_sound] >>
+ match_mp_tac implements_comp_three_refines_term >>
+ METIS_TAC []
+QED
+
+Theorem double_par_intersection1:
+ !omega MS MV S1 S2 S3 x. 
+  x IN S_sem omega MS MV (S_par S1 (S_par S2 S3)) ==>
+  x IN { a INTER b INTER c | a IN S_sem omega MS MV S1 /\
+     b IN S_sem omega MS MV S2 /\ c IN S_sem omega MS MV S3 }
+Proof
+ rw [S_sem,double_intersection] >>
+ Q.EXISTS_TAC `a` >>
+ Q.EXISTS_TAC `a'` >>
+ Q.EXISTS_TAC `b'` >>
+ rw [] >> 
+ METIS_TAC [INTER_ASSOC]
+QED
+
+Theorem double_par_intersection2:
+ !omega MS MV S1 S2 S3 x. 
+  x IN { a INTER b INTER c | a IN S_sem omega MS MV S1 /\
+     b IN S_sem omega MS MV S2 /\ c IN S_sem omega MS MV S3 } ==>
+  x IN S_sem omega MS MV (S_par S1 (S_par S2 S3))
+Proof
+ rw [S_sem,double_intersection] >>
+ Q.EXISTS_TAC `a` >>
+ Q.EXISTS_TAC `b INTER c` >>
+ rw [] >- METIS_TAC [INTER_ASSOC] >>
+ Q.EXISTS_TAC `b` >>
+ Q.EXISTS_TAC `c` >>
+ rw []
+QED
+
+Theorem double_par_intersection:
+ !omega MS MV S1 S2 S3. 
+  S_sem omega MS MV (S_par S1 (S_par S2 S3)) =
+   { a INTER b INTER c | a IN S_sem omega MS MV S1 /\
+     b IN S_sem omega MS MV S2 /\ c IN S_sem omega MS MV S3 }
+Proof
+ rw [] >>
+ once_rewrite_tac [EXTENSION] >>
+ METIS_TAC [double_par_intersection1,double_par_intersection2]
 QED
 
 val _ = export_theory ();
