semantics/compSpecExampleScript.sml
@@ -1,0 +1,598 @@
+open HolKernel boolLib Parse bossLib;
+open pred_setTheory listTheory combinTheory;
+open ottTheory compSpecUtilityTheory compSpecTheory compSpecMetaTheory;
+
+val _ = new_theory "compSpecExample";
+
+Definition example_implements:
+ example_implements c1 c2 A G =
+  P_implements (c_comp c1 c2) (S_assume A G)
+End
+
+(* EVAL ``P_sem omega Mc MS Mq MV (example_implements c1 c2 A G)`` *)
+
+Definition example_4_MS:
+ (example_4_MS s =
+  if s = "S1"
+  then {{(0, 0, 0); (0, 0, 1)}; {(0, 1, 0); (0, 1, 1)}}
+  else if s = "S2"
+  then {{(0, 1, 0); (0, 1, 1)}; {(0, 1, 0); (1, 1, 0)}}
+  else {})
+End
+
+Definition example_5_Mc:
+ (example_5_Mc s =
+  if s = "c3"
+  then {(0, 0, 0); (0, 0, 1)}
+  else if s = "c4"
+  then {(0, 1, 0); (0, 1, 1)}
+  else if s = "c5"
+  then {(0, 1, 0); (1, 1, 0)}
+  else {})
+End
+
+Theorem example_5_c3_S1:
+ !Mq MV. P_sem UNIV example_5_Mc example_4_MS Mq MV (P_implements (c_const "c3") (S_const (Sc_const "S1")))
+Proof
+ rw [P_sem,c_sem,S_sem,example_5_Mc,example_4_MS]
+QED
+
+Theorem example_5_c4_S1:
+ !Mq MV. P_sem UNIV example_5_Mc example_4_MS Mq MV (P_implements (c_const "c4") (S_const (Sc_const "S1")))
+Proof
+ rw [P_sem,c_sem,S_sem,example_5_Mc,example_4_MS]
+QED
+
+Theorem example_5_c3_c4_S1:
+ !Mq MV. ~ (P_sem UNIV example_5_Mc example_4_MS Mq MV
+    (P_implements (c_comp (c_const "c3") (c_const "c4")) (S_const (Sc_const "S1"))))
+Proof
+ rw [P_sem,c_sem,S_sem,example_5_Mc,example_4_MS,INTER_DEF] >-
+  (rw [EXTENSION] >> Q.EXISTS_TAC `(0,0,0)` >> fs []) >>
+ rw [EXTENSION] >>
+ Q.EXISTS_TAC `(0,1,0)` >>
+ fs []
+QED
+
+Theorem example_5_c4_S2:
+ !Mq MV. P_sem UNIV example_5_Mc example_4_MS Mq MV (P_implements (c_const "c4") (S_const (Sc_const "S2")))
+Proof
+ rw [P_sem,c_sem,S_sem,example_5_Mc,example_4_MS]
+QED
+
+Theorem example_5_c5_S2:
+ !Mq MV. P_sem UNIV example_5_Mc example_4_MS Mq MV (P_implements (c_const "c5") (S_const (Sc_const "S2")))
+Proof
+ rw [P_sem,c_sem,S_sem,example_5_Mc,example_4_MS]
+QED
+
+Theorem example_5_c4_c5_S2:
+ !Mq MV. ~ (P_sem UNIV example_5_Mc example_4_MS Mq MV
+    (P_implements (c_comp (c_const "c4") (c_const "c5")) (S_const (Sc_const "S2"))))
+Proof
+ rw [P_sem,c_sem,S_sem,example_5_Mc,example_4_MS,INTER_DEF] >-
+  (rw [EXTENSION] >> Q.EXISTS_TAC `(0,1,1)` >> fs []) >>
+ rw [EXTENSION] >>
+ Q.EXISTS_TAC `(1,1,0)` >>
+ fs []
+QED
+
+Definition P_c_eq_forall_c_assoc:
+ P_c_eq_forall_c_assoc =
+  (P_forall_c "q" (P_forall_c "q'" (P_forall_c "q''"
+     (P_c_eq (c_comp (c_comp (c_var "q") (c_var "q'")) (c_var "q''"))
+             (c_comp (c_var "q") (c_comp (c_var "q'") (c_var "q''")))))))
+End
+
+Theorem P_sem_forall_c_assoc:
+ !omega Mc MS Mq MV.
+   P_sem omega Mc MS Mq MV P_c_eq_forall_c_assoc
+Proof
+ rw [P_c_eq_forall_c_assoc,P_sem,c_sem_comp_ASSOC]
+QED
+
+Definition P_S_eq_forall_S_conj_comm:
+ P_S_eq_forall_S_conj_comm S1 S2 =
+  (P_S_eq (S_conj S1 S2) (S_conj S2 S1))
+End
+
+Theorem P_sem_S_eq_forall_S_conj_comm:
+ !S1 S2 omega Mc MS Mq MV. P_sem omega Mc MS Mq MV (P_S_eq_forall_S_conj_comm S1 S2)
+Proof
+ rw [P_S_eq_forall_S_conj_comm,P_sem,S_sem_conj_COMM]
+QED
+
+Definition P_S_eq_conj_comm_assoc_compat:
+ P_S_eq_conj_comm_assoc_compat S1 S2 =
+  (P_S_eq
+   (S_conj S2 (S_conj S1 (S_const Sc_compat)))
+   (S_conj (S_conj S1 S2) (S_const Sc_compat)))
+End
+
+Theorem P_sem_S_eq_conj_comm_assoc_compat:
+ !S1 S2 omega Mc MS Mq MV. P_sem omega Mc MS Mq MV (P_S_eq_conj_comm_assoc_compat S1 S2)
+Proof
+ rw [P_S_eq_conj_comm_assoc_compat,P_sem,GSYM S_sem_conj_ASSOC] >>
+ rw [S_sem_conj_ASSOC] >>
+ rw [S_sem] >>
+ METIS_TAC [INTER_COMM] 
+QED
+
+Definition example_Gamma:
+ example_Gamma A A1 A2 G G1 G2 =
+  { P_asserts A; P_refines A A1; P_refines (S_conj A G1) A2; P_refines G2 G }
+End
+
+Definition example_Gamma_ext:
+ example_Gamma_ext A A1 A2 A3 G G1 G2 G3 =
+  { P_asserts A;
+    P_refines A A1;
+    P_refines (S_conj A G1) A2;
+    P_refines (S_conj A1 G2) A3;
+    P_refines G3 G }
+End
+
+Definition example_Ps:
+ example_Ps A A1 A2 G G1 G2 =
+  P_S_eq_conj_comm_assoc_compat G1 A INSERT
+  P_S_eq_forall_S_conj_comm A G1 INSERT
+  P_c_eq_forall_c_assoc INSERT
+  example_Gamma A A1 A2 G G1 G2
+End
+
+Definition example_goal:
+ example_goal A A1 A2 G G1 G2 =
+  P_forall_c "q" (P_implies
+   (P_implements (c_var "q") (S_assume (S_conj A1 (S_const Sc_compat)) (S_conj G1 (S_const Sc_compat))))
+   (P_forall_c "q'" (P_implies
+     (P_implements (c_var "q'") (S_assume (S_conj A2 (S_const Sc_compat)) (S_conj G2 (S_const Sc_compat))))
+     (P_implements (c_comp (c_var "q") (c_var "q'"))
+        (S_assume (S_conj A (S_const Sc_compat)) (S_conj G (S_const Sc_compat)))))))
+End
+
+Definition example_goal_ext:
+ example_goal_ext A A1 A2 A3 G G1 G2 G3 =
+  P_forall_c "q" (P_implies
+   (P_implements (c_var "q") (S_assume (S_conj A1 (S_const Sc_compat)) (S_conj G1 (S_const Sc_compat))))
+   (P_forall_c "q'" (P_implies
+     (P_implements (c_var "q'") (S_assume (S_conj A2 (S_const Sc_compat)) (S_conj G2 (S_const Sc_compat))))
+     (P_forall_c "q''" (P_implies
+       (P_implements (c_var "q''") (S_assume (S_conj A3 (S_const Sc_compat)) (S_conj G3 (S_const Sc_compat))))
+        (P_implements (c_comp (c_var "q") (c_comp (c_var "q'") (c_var "q''")))
+         (S_assume (S_conj A (S_const Sc_compat)) (S_conj G (S_const Sc_compat)))))))))
+End
+
+Theorem SUBSET_INTER_POW[local]:
+ !s1 s2 s. s1 SUBSET s /\ s2 SUBSET s ==>
+  s1 INTER s2 IN POW s
+Proof
+ rw [INTER_DEF,SUBSET_DEF,POW_DEF]
+QED
+
+Theorem example_refine_sem:
+ !omega Mc MS Mq MV. 
+ (!s. Mc s SUBSET omega) /\
+ (!s. Mq s SUBSET omega) /\
+ (!s. MS s SUBSET POW omega) /\
+ (!s. MV s SUBSET POW omega) ==>
+ !A A1 A2 G G1 G2.
+ (!P0. P0 IN example_Ps A A1 A2 G G1 G2 ==> P_sem omega Mc MS Mq MV P0) ==>
+ P_sem omega Mc MS Mq MV (example_goal A A1 A2 G G1 G2)
+Proof
+ rw [example_Ps,example_goal,example_Gamma] >>
+
+ `P_sem omega Mc MS Mq MV (P_asserts A)` by METIS_TAC [] >>
+ `P_sem omega Mc MS Mq MV (P_refines A A1)` by METIS_TAC [] >>
+ `P_sem omega Mc MS Mq MV (P_refines (S_conj A G1) A2)` by METIS_TAC [] >>
+ `P_sem omega Mc MS Mq MV (P_refines G2 G)` by METIS_TAC [] >>
+
+ Q.PAT_X_ASSUM `!P0. P` (fn thm => ALL_TAC) >> 
+ fs [P_sem,S_sem,c_sem,downward_closed] >> rw [APPLY_UPDATE_THM] >-
+ METIS_TAC [SUBSET_INTER_POW] >>
+
+ `B' IN S_sem omega MS MV A1` by METIS_TAC [SUBSET_DEF] >>
+ `B' IN POW omega` by METIS_TAC [POW_DEF,SUBSET_DEF] >>
+ 
+ `qs INTER B' IN S_sem omega MS MV G1` by METIS_TAC [] >>
+ `qs INTER B' <> {}` by METIS_TAC [] >>
+ `qs INTER B' IN POW omega` by METIS_TAC [] >>
+ `qs INTER B' IN S_sem omega MS MV A2` by
+   (`qs INTER B' IN S_sem omega MS MV A INTER S_sem omega MS MV G1`
+      suffices_by METIS_TAC [SUBSET_DEF] >>
+    `!e'. e' SUBSET B' ==> e' IN S_sem omega MS MV A` by METIS_TAC [] >>
+    `qs INTER B' SUBSET B'` by rw [INTER_DEF,SUBSET_DEF] >>
+    `qs INTER B' IN S_sem omega MS MV A` by METIS_TAC [] >>
+    METIS_TAC [IN_INTER]) >| [
+
+    `qs' INTER (qs INTER B') IN S_sem omega MS MV G`
+     by METIS_TAC [SUBSET_DEF] >>
+    METIS_TAC [INTER_COMM,INTER_ASSOC],
+
+    
+    `qs' INTER (qs INTER B') IN POW omega`
+     by METIS_TAC [SUBSET_DEF] >>
+    METIS_TAC [INTER_COMM,INTER_ASSOC],
+
+    `qs' INTER (qs INTER B') <> {}`
+      by METIS_TAC [SUBSET_DEF] >>
+    METIS_TAC [INTER_COMM,INTER_ASSOC]
+ ]
+QED
+
+Theorem example_refine_sem_ext[local]:
+ !omega Mc MS Mq MV. 
+ (!s. Mc s SUBSET omega) /\
+ (!s. Mq s SUBSET omega) /\
+ (!s. MS s SUBSET POW omega) /\
+ (!s. MV s SUBSET POW omega) ==>
+ !A A1 A2 A3 G G1 G2 G3.
+ (!P0. P0 IN example_Gamma_ext A A1 A2 A3 G G1 G2 G3 ==> P_sem omega Mc MS Mq MV P0) ==>
+ P_sem omega Mc MS Mq MV (example_goal_ext A A1 A2 A3 G G1 G2 G3)
+Proof
+ rw [example_Gamma_ext,example_goal_ext] >> 
+
+ `P_sem omega Mc MS Mq MV (P_asserts A)` by METIS_TAC [] >>
+ `P_sem omega Mc MS Mq MV (P_refines A A1)` by METIS_TAC [] >>
+ `P_sem omega Mc MS Mq MV (P_refines (S_conj A G1) A2)` by METIS_TAC [] >>
+ `P_sem omega Mc MS Mq MV (P_refines (S_conj A1 G2) A3)` by METIS_TAC [] >>
+ `P_sem omega Mc MS Mq MV (P_refines G3 G)` by METIS_TAC [] >>
+
+ Q.PAT_X_ASSUM `!P0. P` (fn thm => ALL_TAC) >> 
+
+ fs [P_sem,S_sem,c_sem,downward_closed] >> rw [APPLY_UPDATE_THM] >-
+ cheat >| [
+
+  `B' IN S_sem omega MS MV A1` by METIS_TAC [SUBSET_DEF] >>
+  `B' IN POW omega` by METIS_TAC [POW_DEF,SUBSET_DEF] >>
+ 
+  `qs INTER B' IN S_sem omega MS MV G1` by METIS_TAC [] >>
+  `qs INTER B' <> {}` by METIS_TAC [] >>
+
+  `!e'. e' SUBSET B' ==> e' IN S_sem omega MS MV A` by METIS_TAC [] >>
+  `qs INTER B' SUBSET B'` by rw [INTER_DEF,SUBSET_DEF] >>
+  `qs INTER B' IN S_sem omega MS MV A` by METIS_TAC [] >>
+  
+  cheat,
+
+  cheat,
+
+  cheat
+]
+QED
+
+Theorem ax_IN:
+ !P G. P IN G ==> spec_holds G P
+Proof
+ rw [] >> 
+ sg `?G'. G = P INSERT G'` >-
+  (Q.EXISTS_TAC `G DELETE P` >>
+   rw [INSERT_DELETE]) >>
+ rw [] >> MATCH_MP_TAC ax >> rw [clause_name_def]
+QED
+
+Theorem SVARIANT_INSERT:
+ !s x. FINITE s ==> SVARIANT (x INSERT s) <> x
+Proof
+ rw [] >>
+ strip_tac >>
+ `FINITE (x INSERT s)` by rw [FINITE_INSERT] >>
+ `SVARIANT (x INSERT s) NOTIN (x INSERT s)` by
+  METIS_TAC [SVARIANT_FINITE] >>
+ fs []
+QED
+
+Theorem FINITE_example_Ps:
+ !A A1 A2 G G1 G2.
+  FINITE (example_Ps A A1 A2 G G1 G2)
+Proof
+ rw [example_Ps,example_Gamma]
+QED
+
+Theorem fv_P_c_P_c_eq_forall_c_assoc_EMPTY:
+ fv_P_c P_c_eq_forall_c_assoc = {}
+Proof
+ rw [fv_P_c,P_c_eq_forall_c_assoc,fv_c,UNION_DEF,DELETE_DEF,DIFF_DEF,EXTENSION] >>
+ METIS_TAC []
+QED
+
+Theorem fv_P_c_P_S_eq_forall_S_conj_comm_EMPTY:
+ !S1 S2. fv_P_c (P_S_eq_forall_S_conj_comm S1 S2) = {}
+Proof
+ rw [fv_P_c,P_S_eq_forall_S_conj_comm]
+QED
+
+Theorem fv_P_c_P_S_eq_conj_comm_assoc_compat_EMPTY:
+ !S1 S2. fv_P_c (P_S_eq_conj_comm_assoc_compat S1 S2) = {}
+Proof
+ rw [fv_P_c,P_S_eq_conj_comm_assoc_compat]
+QED
+
+Theorem fv_P_S_P_S_eq_forall_S_conj_comm_EMPTY:
+ !S1 S2. fv_P_S (P_S_eq_forall_S_conj_comm S1 S2) = fv_S S1 UNION fv_S S2
+Proof
+ rw [fv_P_S,P_S_eq_forall_S_conj_comm,fv_S,UNION_DEF,EXTENSION] >>
+ METIS_TAC []
+QED
+
+Theorem fv_P_S_P_S_eq_conj_comm_assoc_compat_UNION:
+ !S1 S2. fv_P_S (P_S_eq_conj_comm_assoc_compat S1 S2) = fv_S S1 UNION fv_S S2
+Proof
+ rw [fv_P_S,P_S_eq_conj_comm_assoc_compat,fv_S,UNION_DEF,EXTENSION] >>
+ METIS_TAC []
+QED
+
+Theorem BIGUNION_IMAGE_f_NOTIN:
+ !x f G.
+  (x NOTIN BIGUNION (IMAGE f G))
+  <=>
+  (!P. P IN G ==> x NOTIN (f P))
+Proof
+ rw [] >> METIS_TAC []
+QED
+
+Theorem example_Gamma_fv_P_c_NOTIN:
+ !A A1 A2 G G1 G2 P.
+  P IN example_Gamma A A1 A2 G G1 G2 ==>
+  fv_P_c P = {}
+Proof
+ rw [example_Gamma] >> rw [fv_P_c]
+QED
+
+Theorem example_Gamma_fv_P_S:
+ !A A1 A2 G G1 G2 P.
+  BIGUNION (IMAGE fv_P_S (example_Gamma A A1 A2 G G1 G2)) =
+  (fv_S A UNION fv_S A1 UNION fv_S A2 UNION fv_S G UNION fv_S G1 UNION fv_S G2)
+Proof
+ rw [example_Gamma] >> rw [fv_P_S,fv_S] >> rw [UNION_DEF,EXTENSION] >> METIS_TAC []
+QED
+
+Theorem example_Gamma_fv_P_c_empty:
+ !A A1 A2 G G1 G2 x.
+  IMAGE fv_P_c (example_Gamma A A1 A2 G G1 G2) = {{}}
+Proof
+ rw [example_Gamma,fv_P_c]
+QED
+
+Theorem example_Ps_fv_P_c_NOTIN:
+ !A A1 A2 G G1 G2 x. x NOTIN BIGUNION (IMAGE fv_P_c (example_Ps A A1 A2 G G1 G2))
+Proof
+ rw [BIGUNION_IMAGE_f_NOTIN,example_Ps] >-
+ METIS_TAC [NOT_IN_EMPTY,fv_P_c_P_S_eq_conj_comm_assoc_compat_EMPTY] >-
+ METIS_TAC [NOT_IN_EMPTY,fv_P_c_P_S_eq_forall_S_conj_comm_EMPTY] >-
+ METIS_TAC [NOT_IN_EMPTY,fv_P_c_P_c_eq_forall_c_assoc_EMPTY] >> 
+ METIS_TAC [example_Gamma_fv_P_c_NOTIN,NOT_IN_EMPTY]
+QED
+
+Theorem example_Ps_INSERT_fv_P_c_NOTIN:
+ !A A1 A2 G G1 G2 q q'.
+  q <> q' ==>
+  q' NOTIN BIGUNION (IMAGE fv_P_c
+   (P_implements (c_var q)
+   (S_assume (S_conj A1 (S_const Sc_compat))
+             (S_conj G1 (S_const Sc_compat))) INSERT
+   example_Ps A A1 A2 G G1 G2))
+Proof
+ rw [BIGUNION_IMAGE_f_NOTIN,example_Ps] >-
+ rw [fv_P_c,fv_c] >-
+ METIS_TAC [NOT_IN_EMPTY,fv_P_c_P_S_eq_conj_comm_assoc_compat_EMPTY] >-
+ METIS_TAC [NOT_IN_EMPTY,fv_P_c_P_S_eq_forall_S_conj_comm_EMPTY] >-
+ METIS_TAC [NOT_IN_EMPTY,fv_P_c_P_c_eq_forall_c_assoc_EMPTY] >> 
+ METIS_TAC [example_Gamma_fv_P_c_NOTIN,NOT_IN_EMPTY]
+QED
+
+Theorem example_Ps_INSERT_INSERT_fv_P_c_NOTIN:
+ !A A1 A2 G G1 G2 q q' q0.
+  q <> q0 /\ q' <> q0 ==> 
+  q0 NOTIN BIGUNION (IMAGE fv_P_c
+   ((P_implements (c_var q')
+   (S_assume (S_conj A2 (S_const Sc_compat))
+             (S_conj G2 (S_const Sc_compat)))) INSERT
+   (P_implements (c_var q)
+   (S_assume (S_conj A1 (S_const Sc_compat))
+             (S_conj G1 (S_const Sc_compat)))) INSERT
+   example_Ps A A1 A2 G G1 G2))
+Proof
+ rw [BIGUNION_IMAGE_f_NOTIN,example_Ps] >>
+ rw [fv_P_c,fv_c] >-
+ METIS_TAC [NOT_IN_EMPTY,fv_P_c_P_S_eq_conj_comm_assoc_compat_EMPTY] >-
+ METIS_TAC [NOT_IN_EMPTY,fv_P_c_P_S_eq_forall_S_conj_comm_EMPTY] >-
+ METIS_TAC [NOT_IN_EMPTY,fv_P_c_P_c_eq_forall_c_assoc_EMPTY] >> 
+ METIS_TAC [example_Gamma_fv_P_c_NOTIN,NOT_IN_EMPTY]
+QED
+
+Theorem Ssubst_SVARIANT_fv_S:
+ !S S' VS. 
+  FINITE VS /\ fv_S S SUBSET VS ==>
+  Ssubst_S ((SVARIANT VS =+ S') S_var) S = S
+Proof
+ Induct >>  rw [Ssubst_S,fv_S] >>
+ rw [APPLY_UPDATE_THM] >>
+ METIS_TAC [SVARIANT_FINITE]
+QED
+
+Theorem example_refine_spec_holds:
+ !A A1 A2 G G1 G2.
+ spec_holds
+  (example_Ps A A1 A2 G G1 G2)
+  (example_goal A A1 A2 G G1 G2)
+Proof
+ rw [example_goal] >>
+
+ MATCH_MP_TAC all_in_c >>
+ Q.EXISTS_TAC `"q1"` >>
+ rw [clause_name_def,example_Ps_fv_P_c_NOTIN] >-
+ rw [fv_P_c,fv_c] >>
+ rw [csubst_P] >-
+ (fs [fv_P_c,fv_c] >> rw [] >> fs [APPLY_UPDATE_THM,fv_c]) >>
+ PAT_X_ASSUM ``~ ?y. P`` (fn thm => ALL_TAC) >>
+ rw [csubst_c,APPLY_UPDATE_THM] >>
+
+ MATCH_MP_TAC imp_in >>
+ rw [clause_name_def] >>
+
+ MATCH_MP_TAC all_in_c >>
+ Q.EXISTS_TAC `"q2"` >>
+
+ rw [clause_name_def,example_Ps_INSERT_fv_P_c_NOTIN] >-
+ rw [fv_P_c,fv_c] >>
+ rw [csubst_P,csubst_c,APPLY_UPDATE_THM] >>
+
+ MATCH_MP_TAC imp_in >>
+ rw [clause_name_def] >>
+
+ MATCH_MP_TAC cont_in >>
+
+ Q.EXISTS_TAC `"q"` >>
+ rw [clause_name_def,fv_c] >>
+
+ MATCH_MP_TAC all_in_c >>
+ Q.EXISTS_TAC `"q0"` >>
+
+ rw [clause_name_def,example_Ps_INSERT_INSERT_fv_P_c_NOTIN] >-
+ rw [fv_P_c,fv_c] >>
+ rw [csubst_P,csubst_c,APPLY_UPDATE_THM] >>
+
+ MATCH_MP_TAC imp_in >>
+ rw [clause_name_def] >>
+
+ MATCH_MP_TAC cr >>
+ Q.EXISTS_TAC `G2` >>
+
+ rw [clause_name_def] >-
+  (Q.ABBREV_TAC `Gamma = P_implements (c_var "q0") (S_conj A (S_const Sc_compat)) INSERT
+      P_implements (c_var "q2")
+        (S_assume (S_conj A2 (S_const Sc_compat))
+           (S_conj G2 (S_const Sc_compat))) INSERT
+      P_implements (c_var "q1")
+        (S_assume (S_conj A1 (S_const Sc_compat))
+           (S_conj G1 (S_const Sc_compat))) INSERT example_Ps A A1 A2 G G1 G2` >>
+  `spec_holds Gamma (csubst_P
+    (("q" =+ (c_comp (c_var "q0") (c_comp (c_var "q1") (c_var "q2")))) c_var)
+     (P_implements (c_var "q") (S_conj G2 (S_const Sc_compat))))`
+   suffices_by rw [csubst_P,csubst_c] >>
+  
+  MATCH_MP_TAC eq_el_c >>
+  
+  Q.EXISTS_TAC `c_comp (c_comp (c_var "q0") (c_var "q1")) (c_var "q2")` >>
+  rw [clause_name_def] >-
+   (`spec_holds Gamma
+      (csubst_P (("q''" =+ (c_var "q2")) c_var)
+        (P_c_eq (c_comp (c_comp (c_var "q0") (c_var "q1")) (c_var "q''"))
+                (c_comp (c_var "q0") (c_comp (c_var "q1") (c_var "q''")))))`
+      suffices_by rw [csubst_P,csubst_c,APPLY_UPDATE_THM] >>
+
+    MATCH_MP_TAC all_el_c >>
+    rw [clause_name_def] >>
+    
+    `spec_holds Gamma
+      (csubst_P (("q'" =+ (c_var "q1")) c_var)
+        (P_forall_c "q''" 
+           (P_c_eq
+                (c_comp (c_comp (c_var "q0") (c_var "q'")) (c_var "q''"))
+                (c_comp (c_var "q0") (c_comp (c_var "q'") (c_var "q''"))))))`
+      suffices_by rw [csubst_P,csubst_c,APPLY_UPDATE_THM,fv_P_c,fv_c] >>
+
+    MATCH_MP_TAC all_el_c >>
+    rw [clause_name_def] >>
+
+    `spec_holds Gamma
+      (csubst_P (("q" =+ (c_var "q0")) c_var)
+       (P_forall_c "q'"
+         (P_forall_c "q''"
+           (P_c_eq
+            (c_comp (c_comp (c_var "q") (c_var "q'")) (c_var "q''"))
+            (c_comp (c_var "q") (c_comp (c_var "q'") (c_var "q''")))))))`
+      suffices_by rw [csubst_P,csubst_c,APPLY_UPDATE_THM,fv_P_c,fv_c] >>
+
+    MATCH_MP_TAC all_el_c >>
+    rw [clause_name_def] >>
+    
+    match_mp_tac ax_IN >>
+    rw [Abbr `Gamma`, example_Ps,example_Gamma,P_c_eq_forall_c_assoc]) >>
+  
+  rw [csubst_P,csubst_c] >>
+
+  MATCH_MP_TAC cont_el >>
+  Q.EXISTS_TAC `S_conj A2 (S_const Sc_compat)` >>
+  rw [clause_name_def] >-
+   (MATCH_MP_TAC cr >>
+    Q.EXISTS_TAC `S_conj G1 A` >>
+    rw [clause_name_def] >-
+     (`spec_holds Gamma
+       (Ssubst_P (("V" =+ S_conj (S_conj G1 A) (S_const Sc_compat)) S_var)
+         (P_implements (c_comp (c_var "q0") (c_var "q1")) (S_var "V")))`
+       suffices_by rw [Ssubst_P,Ssubst_S] >>
+      
+      MATCH_MP_TAC eq_el_S >>
+      rw [clause_name_def] >>
+
+      Q.EXISTS_TAC `S_conj A (S_conj G1 (S_const Sc_compat))` >>
+      rw [Ssubst_P,Ssubst_S,APPLY_UPDATE_THM] >-
+       (match_mp_tac ax_IN >>
+        rw [Abbr `Gamma`, example_Ps,example_Gamma,P_S_eq_conj_comm_assoc_compat]) >>
+
+      MATCH_MP_TAC conj_in >>
+      rw [clause_name_def] >-
+       (MATCH_MP_TAC assn_el >>
+        rw [clause_name_def] >-
+         (match_mp_tac ax_IN >>
+          rw [Abbr `Gamma`, example_Ps,example_Gamma]) >>
+        MATCH_MP_TAC conj_el1 >>
+        Q.EXISTS_TAC `S_const (Sc_compat)` >>
+        rw [clause_name_def] >>
+        match_mp_tac ax_IN >>
+        rw [Abbr `Gamma`, example_Ps,example_Gamma]) >>
+      MATCH_MP_TAC cont_el >>
+      Q.EXISTS_TAC `S_conj A1 (S_const Sc_compat)` >>
+      rw [clause_name_def] >-
+       (MATCH_MP_TAC cr >>
+        Q.EXISTS_TAC `A` >>
+        rw [clause_name_def] >>
+        match_mp_tac ax_IN >>
+        rw [Abbr `Gamma`, example_Ps,example_Gamma]) >>
+      match_mp_tac ax_IN >>
+      rw [Abbr `Gamma`, example_Ps,example_Gamma]) >>
+
+    `!S. Ssubst_S S_var⦇SVARIANT (fv_S A2) ↦ S⦈ A2 = A2`
+     by (MATCH_MP_TAC Ssubst_SVARIANT_fv_S >> fs [FINITE_fv_S]) >>
+
+    `spec_holds Gamma (Ssubst_P
+      ((SVARIANT (fv_S A2) =+ S_conj G1 A) S_var) (P_refines (S_var (SVARIANT (fv_S A2))) A2))`
+     suffices_by (rw [Ssubst_P,Ssubst_S,APPLY_UPDATE_THM]) >>
+
+    MATCH_MP_TAC eq_el_S >>
+    Q.EXISTS_TAC `S_conj A G1` >>
+
+    rw [clause_name_def] >-
+     (match_mp_tac ax_IN >> rw [Abbr `Gamma`,example_Ps,example_Gamma,P_S_eq_forall_S_conj_comm]) >>
+    rw [Ssubst_P,Ssubst_S] >>
+    match_mp_tac ax_IN >>
+    rw [Abbr `Gamma`,example_Ps,example_Gamma]) >>
+   match_mp_tac ax_IN >>
+   rw [Abbr `Gamma`,example_Ps,example_Gamma]) >>
+ match_mp_tac ax_IN >>
+ rw [example_Ps,example_Gamma]
+QED
+
+Theorem example_refine_sem_spec_holds:
+ !omega Mc MS Mq MV. 
+ (!s. Mc s SUBSET omega) /\
+ (!s. Mq s SUBSET omega) /\
+ (!s. MS s SUBSET POW omega) /\
+ (!s. MV s SUBSET POW omega) ==>
+ !A A1 A2 G G1 G2.
+ (!P0. P0 IN example_Ps A A1 A2 G G1 G2 ==> P_sem omega Mc MS Mq MV P0) ==>
+ P_sem omega Mc MS Mq MV (example_goal A A1 A2 G G1 G2)
+Proof
+ rw [] >>
+ `spec_system_sound spec_holds omega`
+  by rw [spec_holds_system_sound] >>
+ `spec_holds (example_Ps A A1 A2 G G1 G2) (example_goal A A1 A2 G G1 G2)`
+  by METIS_TAC [example_refine_spec_holds] >>
+ fs [spec_system_sound] >>
+ METIS_TAC []
+QED
+
+(* FIXME: express example_goal in FOL *)
+
+val _ = export_theory ();
