semantics/compSpecMitlFLDScript.sml
@@ -1,0 +1,90 @@
+open HolKernel boolLib Parse bossLib pred_setTheory listTheory;
+open combinTheory arithmeticTheory realTheory RealArith realSimps;
+open ottTheory compSpecUtilityTheory compSpecTheory compSpecMetaTheory;
+open mitlTheory compSpecMitlTheory;
+
+val _ = new_theory "compSpecMitlFLD";
+
+Datatype:
+ var_FLD = Var_Avout | Var_Avin | Var_Al | Var_Dl
+End
+
+Datatype:
+ val_FLD = Val_num num | Val_real real
+End
+
+Type state_FLD = ``:var_FLD -> val_FLD``
+
+Datatype:
+ exp_FLD = exp_EQ var_FLD val_FLD | exp_LT var_FLD val_FLD | exp_GT var_FLD val_FLD
+  | exp_AND exp_FLD exp_FLD | exp_OR exp_FLD exp_FLD | exp_NOT exp_FLD
+End
+
+Definition state_holds_FLD:
+ (state_holds_FLD (s:state_FLD) (exp_EQ var val) : bool =
+  (s var = val))
+ /\
+ (state_holds_FLD (s:state_FLD) (exp_LT Var_Avout (Val_real r)) : bool =
+  (case s Var_Avout of Val_real r' => r < r' | _ => F))
+ /\
+ (state_holds_FLD (s:state_FLD) (exp_LT Var_Avin (Val_real r)) : bool =
+  (case s Var_Avin of Val_real r' => r < r' | _ => F))
+ /\
+ (state_holds_FLD (s:state_FLD) (exp_LT Var_Al (Val_num n)) : bool =
+  (case s Var_Al of Val_num n' => n < n' | _ => F))
+ /\
+ (state_holds_FLD (s:state_FLD) (exp_LT Var_Dl (Val_num n)) : bool =
+  (case s Var_Dl of Val_num n' => n < n' | _ => F))
+ /\
+ (state_holds_FLD (s:state_FLD) (exp_GT Var_Avout (Val_real r)) : bool =
+  (case s Var_Avout of Val_real r' => r > r' | _ => F))
+ /\
+ (state_holds_FLD (s:state_FLD) (exp_GT Var_Avin (Val_real r)) : bool =
+  (case s Var_Avin of Val_real r' => r > r' | _ => F))
+ /\
+ (state_holds_FLD (s:state_FLD) (exp_GT Var_Al (Val_num n)) : bool =
+  (case s Var_Al of Val_num n' => n > n' | _ => F))
+ /\
+ (state_holds_FLD (s:state_FLD) (exp_GT Var_Dl (Val_num n)) : bool =
+  (case s Var_Dl of Val_num n' => n > n' | _ => F))
+ /\
+ (state_holds_FLD (s:state_FLD) (exp_AND e1 e2) : bool =
+  (state_holds_FLD s e1 /\ state_holds_FLD s e2))
+ /\
+ (state_holds_FLD (s:state_FLD) (exp_OR e1 e2) : bool =
+  (state_holds_FLD s e1 \/ state_holds_FLD s e2))
+ /\
+ (state_holds_FLD (s:state_FLD) (exp_NOT e) : bool =
+  (~ state_holds_FLD s e))
+End
+
+Type timed_word_FLD = ``:(num -> (state_FLD # real))``
+
+Definition omega_FLD:
+ omega_FLD : timed_word_FLD set =
+  { tau |     
+    (!i j. i < j ==> (SND (tau i)) < (SND (tau j)))
+    /\
+    (!i. ?r. (FST (tau i)) Var_Avout = Val_real r)
+    /\
+    (!i. ?r. (FST (tau i)) Var_Avin = Val_real r)
+    /\
+    (!i. ?n. (FST (tau i)) Var_Al = Val_num n)
+    /\
+    (!i. ?n. (FST (tau i)) Var_Dl = Val_num n)
+  }
+End
+
+Theorem omega_FLD_suffix:
+ !tau. tau IN omega_FLD ==>
+ !i. timed_word_suffix tau i IN omega_FLD
+Proof
+ rw [omega_FLD,timed_word_suffix]
+QED
+
+Definition spec_temporal_holds_FLD_def:
+ spec_temporal_holds_FLD : (exp_FLD Pt -> bool) -> exp_FLD Pt -> bool = 
+  spec_temporal_holds
+End
+
+val _ = export_theory ();
