semantics/compSpecMitlScript.sml
@@ -1,0 +1,133 @@
+open HolKernel boolLib Parse bossLib pred_setTheory listTheory;
+open combinTheory arithmeticTheory realTheory RealArith realSimps;
+open ottTheory compSpecUtilityTheory compSpecTheory compSpecMetaTheory mitlTheory;
+
+val _ = new_theory "compSpecMitl";
+
+Definition St_sem:
+ (St_sem state_holds omega MS MV (St_const (T_const sn)) = MS sn)
+ /\
+ (St_sem state_holds omega MS MV (St_conj S1 S2) =
+   St_sem state_holds omega MS MV S1 INTER St_sem state_holds omega MS MV S2)
+ /\
+ (St_sem state_holds omega MS MV (St_assume S1 S2) =
+  { B | B IN POW omega /\
+    !B'. B' IN St_sem state_holds omega MS MV S1 ==> B INTER B' IN St_sem state_holds omega MS MV S2 })
+ /\
+ (St_sem state_holds omega MS MV (St_par S1 S2) =
+  double_intersection (St_sem state_holds omega MS MV S1) (St_sem state_holds omega MS MV S2))
+ /\
+ (St_sem state_holds omega MS MV (St_var sn) = MV sn)
+ /\
+ (St_sem state_holds omega MS MV (St_const T_compat) = { B | B IN POW omega /\ B <> {} })
+ /\
+ (St_sem state_holds omega MS MV (St_const T_top) = { omega })
+ /\
+ (St_sem state_holds omega MS MV (St_const (T_hat f)) = POW (mitl_general_sem state_holds omega 0 f))
+End
+
+Definition Pt_sem:
+ (Pt_sem state_holds omega Mc MS Mq MV (Pt_implements c S) =
+  (c_sem Mc Mq c IN St_sem state_holds omega MS MV S))
+ /\
+ (Pt_sem state_holds omega Mc MS Mq MV (Pt_refines S1 S2) =
+  (St_sem state_holds omega MS MV S1 SUBSET St_sem state_holds omega MS MV S2))
+ /\
+ (Pt_sem state_holds omega Mc MS Mq MV (Pt_asserts S) =
+  (downward_closed (St_sem state_holds omega MS MV S)))
+ /\
+ (Pt_sem state_holds omega Mc MS Mq MV (Pt_forall_c q P) =
+  (!qs. Pt_sem state_holds omega Mc MS ((q =+ qs) Mq) MV P))
+ /\
+ (Pt_sem state_holds omega Mc MS Mq MV (Pt_exists_c q P) =
+  (?qs. Pt_sem state_holds omega Mc MS ((q =+ qs) Mq) MV P))
+ /\
+ (Pt_sem state_holds omega Mc MS Mq MV (Pt_forall_St Vv P) =
+  (!Vs. Pt_sem state_holds omega Mc MS Mq ((Vv =+ Vs) MV) P))
+ /\
+ (Pt_sem state_holds omega Mc MS Mq MV (Pt_exists_St Vv P) =
+  (?Vs. Pt_sem state_holds omega Mc MS Mq ((Vv =+ Vs) MV) P))
+ /\
+ (Pt_sem state_holds omega Mc MS Mq MV (Pt_implies P1 P2) =
+  (Pt_sem state_holds omega Mc MS Mq MV P1 ==> Pt_sem state_holds omega Mc MS Mq MV P2))
+ /\
+ (Pt_sem state_holds omega Mc MS Mq MV (Pt_and P1 P2) =
+  (Pt_sem state_holds omega Mc MS Mq MV P1 /\ Pt_sem state_holds omega Mc MS Mq MV P2))
+ /\
+ (Pt_sem state_holds omega Mc MS Mq MV (Pt_not P) =
+  ~(Pt_sem state_holds omega Mc MS Mq MV P))
+ /\
+ (Pt_sem state_holds omega Mc MS Mq MV (Pt_c_eq c1 c2) =
+  (c_sem Mc Mq c1 = c_sem Mc Mq c2)) 
+ /\
+ (Pt_sem state_holds omega Mc MS Mq MV (Pt_St_eq S1 S2) =
+  (St_sem state_holds omega MS MV S1 = St_sem state_holds omega MS MV S2))
+End
+
+Theorem pow_mitl_sem_downward_closed:
+ !state_holds omega fm. downward_closed (POW (mitl_general_sem state_holds omega 0 fm))
+Proof
+ strip_tac >> strip_tac >> Induct >> rw [downward_closed,mitl_general_sem] >>
+ METIS_TAC [SUBSET_DEF,IN_POW]
+QED
+
+Theorem mitl_lift_assertional:
+ !state_holds omega Mc MS Mq MV fm.
+  Pt_sem state_holds omega Mc MS Mq MV (Pt_asserts (St_const (T_hat fm)))
+Proof
+ rw [Pt_sem,St_sem,pow_mitl_sem_downward_closed]
+QED
+
+Inductive spec_temporal_mitl_proof:
+[spec_temporal_mitl:] (!(state_holds:'state -> 'a -> bool) omega (Gt:'a Gt) (fm fm':'a f).
+ (!tau. tau IN omega /\ (!i. timed_word_suffix tau i IN omega) ==> mitl_general_holds state_holds tau 0 (mitl_implies fm fm'))
+ ==>
+ spec_temporal_mitl_holds state_holds omega Gt (Pt_refines (St_const (T_hat fm)) (St_const (T_hat fm'))))
+End
+
+Definition spec_temporal_mitl_system_sound:
+  spec_temporal_mitl_system_sound R (state_holds : 'state -> 'a -> bool) omega =
+  (!Mc MS Mq MV G Pt.
+    (!s. Mc s SUBSET omega) /\
+    (!s. Mq s SUBSET omega) /\
+    (!s. MS s SUBSET POW omega) /\
+    (!s. MV s SUBSET POW omega) /\
+    (!P0. P0 IN G ==> Pt_sem state_holds omega Mc MS Mq MV P0) /\
+    (!tau. tau IN omega ==> (!i. timed_word_suffix tau i IN omega)) /\
+    R state_holds omega G Pt ==>
+    Pt_sem state_holds omega Mc MS Mq MV Pt)
+End
+
+Theorem spec_temporal_mitl_holds_system_sound:
+ !(state_holds : 'state -> 'a -> bool) omega.
+  spec_temporal_mitl_system_sound spec_temporal_mitl_holds state_holds omega
+Proof
+ `!(state_holds : 'state -> 'a -> bool) omega G Pt.
+  spec_temporal_mitl_holds state_holds omega G Pt ==>
+  !Mc Mq MS MV.
+  (!s. Mc s SUBSET omega) /\
+  (!s. Mq s SUBSET omega) /\
+  (!s. MS s SUBSET POW omega) /\
+  (!s. MV s SUBSET POW omega) /\
+  (!P0. P0 IN G ==> Pt_sem state_holds omega Mc MS Mq MV P0) /\
+  (!tau. tau IN omega ==> (!i. timed_word_suffix tau i IN omega)) ==>
+  Pt_sem state_holds omega Mc MS Mq MV Pt`
+  suffices_by METIS_TAC [spec_temporal_mitl_system_sound] >> 
+ ho_match_mp_tac spec_temporal_mitl_proof_ind >> rw [] >| [
+  rw [Pt_sem,St_sem] >>
+  rw [SUBSET_DEF] >>
+  `x SUBSET (mitl_general_sem state_holds omega 0 fm)` by METIS_TAC [IN_POW] >>
+  `x SUBSET (mitl_general_sem state_holds omega 0 fm')` suffices_by METIS_TAC [IN_POW] >>
+  fs [mitl_general_holds] >>
+  `x SUBSET omega` by METIS_TAC [mitl_general_sem_omega,SUBSET_DEF] >>
+  `!y. y IN mitl_general_sem state_holds omega 0 fm /\ y IN omega ==> y IN mitl_general_sem state_holds omega 0 fm'`
+   suffices_by fs [SUBSET_DEF] >>
+  rw [] >>
+  `!i. timed_word_suffix y i IN omega` by METIS_TAC [] >>
+  `mitl_general_holds state_holds y 0 fm` by METIS_TAC [mitl_general_holds_sem] >>
+  `mitl_general_holds state_holds y 0 fm'` by METIS_TAC [] >>
+  METIS_TAC [mitl_general_holds_sem]
+ ]
+QED
+
+val _ = export_theory ();
