semantics/mitlScript.sml
@@ -1,0 +1,349 @@
+open HolKernel boolLib Parse bossLib;
+open pred_setTheory listTheory sumTheory combinTheory stringTheory;
+open arithmeticTheory realTheory RealArith realSimps;
+open compSpecTheory;
+
+val _ = new_theory "mitl";
+
+Definition interval_sem:
+ (interval_sem (interval_closed a b) =
+  { r | &a <= r /\ r <= &b })
+ /\
+ (interval_sem (interval_left_half_open a b) =
+  { r | &a < r /\ r <= &b })
+ /\
+ (interval_sem (interval_right_half_open_num a b) =
+  { r | &a <= r /\ r < &b })
+ /\
+ (interval_sem (interval_right_half_open_inf a) =
+  { r | &a <= r })
+/\
+ (interval_sem (interval_open_num a b) =
+  { r | &a < r /\ r < &b })
+ /\
+ (interval_sem (interval_open_inf a) =
+  { r | &a < r })
+End
+
+Definition interval_pos_shift:
+ (interval_pos_shift (t:real) (interval_closed a b) =
+  { r | r >= 0 /\ t + &a <= r /\ r <= t + &b })
+ /\
+ (interval_pos_shift t (interval_left_half_open a b) =
+  { r | r >= 0 /\ t + &a < r /\ r <= t + &b })
+ /\
+ (interval_pos_shift t (interval_right_half_open_num a b) =
+  { r | r >= 0 /\ t + &a <= r /\ r < t + &b })
+ /\
+ (interval_pos_shift t (interval_right_half_open_inf a) =
+  { r | r >= 0 /\ t + &a <= r })
+ /\
+ (interval_pos_shift t (interval_open_num a b) =
+  { r | r >= 0 /\ t + &a < r /\ r < t + &b })
+ /\
+ (interval_pos_shift t (interval_open_inf a) =
+  { r | r >= 0 /\ t + &a < r })
+End
+
+Definition interval_neg_shift:
+ (interval_neg_shift (t:real) (interval_closed a b) =
+  { r | r >= 0 /\ t - &b <= r /\ r <= t - &a })
+ /\
+ (interval_neg_shift t (interval_left_half_open a b) =
+  { r | r >= 0 /\ t - &b <= r /\ r < t - &a })
+ /\
+ (interval_neg_shift t (interval_right_half_open_num a b) =
+  { r | r >= 0 /\ t - &b < r /\ r <= t - &a })
+ /\
+ (interval_neg_shift t (interval_right_half_open_inf a) =
+  { r | r >= 0 /\ r <= t - &a })
+ /\
+ (interval_neg_shift t (interval_open_num a b) =
+  { r | r >= 0 /\ t - &b < r /\ r < t - &a })
+ /\
+ (interval_neg_shift t (interval_open_inf a) =
+  { r | r >= 0 /\ r < t - &a })
+End
+
+Type timed_word = ``:(num -> ('state # real))``
+
+Definition timed_word_suffix:
+ timed_word_suffix (tau: 'state timed_word) (i:num) : 'state timed_word =
+   \x. tau (i + x)
+End
+
+Definition mitl_general_holds:
+  (mitl_general_holds 
+    (state_holds : 'state -> 'a -> bool)
+    (tau : 'state timed_word)
+    (i : num) (mitl_const p : 'a f) : bool = 
+   state_holds (FST (tau i)) p)
+  /\
+  (mitl_general_holds state_holds tau i (mitl_not f) =
+   ~ mitl_general_holds state_holds tau i f)
+  /\
+  (mitl_general_holds state_holds tau i (mitl_and f f') =
+    (mitl_general_holds state_holds tau i f /\ mitl_general_holds state_holds tau i f'))
+  /\
+  (mitl_general_holds state_holds tau i (mitl_implies f f') =
+    (mitl_general_holds state_holds tau i f ==> mitl_general_holds state_holds tau i f'))
+  /\
+  (mitl_general_holds state_holds tau i (mitl_until f iv f') =
+   (?j. (SND (tau j)) IN interval_pos_shift (SND (tau i)) iv /\
+     mitl_general_holds state_holds tau j f' /\
+     !k. (SND (tau k)) IN { r | (SND (tau i)) <= r /\ r <= (SND (tau j)) } ==>
+      mitl_general_holds state_holds tau k f))
+  /\
+  (mitl_general_holds state_holds tau i (mitl_box iv f) = 
+   (!j. (SND (tau j)) IN interval_pos_shift (SND (tau i)) iv ==>
+     mitl_general_holds state_holds tau j f))
+  /\
+  (mitl_general_holds state_holds tau i (mitl_diamond iv f) =
+   (?j. (SND (tau j)) IN interval_pos_shift (SND (tau i)) iv /\
+     mitl_general_holds state_holds tau j f))
+  /\
+  (mitl_general_holds state_holds tau i (mitl_since f iv f') =
+   (?j. (SND (tau j)) IN interval_neg_shift (SND (tau i)) iv /\
+     mitl_general_holds state_holds tau j f' /\
+     !k. (SND (tau k)) IN { r | (SND (tau j)) <= r /\ r <= (SND (tau i)) } ==> 
+      mitl_general_holds state_holds tau k f))
+  /\
+  (mitl_general_holds state_holds tau i (mitl_box_dash iv f) = 
+   (!j. (SND (tau j)) IN interval_neg_shift (SND (tau i)) iv ==>
+     mitl_general_holds state_holds tau j f))
+  /\
+  (mitl_general_holds state_holds tau i (mitl_diamond_dash iv f) = 
+   (?j. (SND (tau j)) IN interval_neg_shift (SND (tau i)) iv /\
+     mitl_general_holds state_holds tau j f))
+End
+
+Definition mitl_general_sem:
+ (mitl_general_sem
+  (state_holds : 'state -> 'a -> bool)
+  (omega : ('state timed_word) set)
+  (i : num) (mitl_const p : 'a f) : ('state timed_word) set =
+  { tau | tau IN omega /\ state_holds (FST (tau i)) p })
+ /\
+ (mitl_general_sem state_holds omega i (mitl_not dm) =
+  omega DIFF (mitl_general_sem state_holds omega i dm))
+ /\
+ (mitl_general_sem state_holds omega i (mitl_and dm1 dm2) =
+  (mitl_general_sem state_holds omega i dm1) INTER
+   (mitl_general_sem state_holds omega i dm2))
+ /\
+ (mitl_general_sem state_holds omega i (mitl_implies dm1 dm2) =
+  mitl_general_sem state_holds omega i dm2 UNION
+   (omega DIFF mitl_general_sem state_holds omega i dm1))                   
+ /\
+ (mitl_general_sem state_holds omega i (mitl_until dm1 iv dm2) =
+  { tau | tau IN omega /\
+    ?j. (SND (tau j)) IN interval_pos_shift (SND (tau i)) iv /\
+     tau IN mitl_general_sem state_holds omega j dm2 /\ 
+      !k. (SND (tau k)) IN { r | (SND (tau i)) <= r /\ r <= (SND (tau j)) } ==>
+       tau IN mitl_general_sem state_holds omega k dm1 })
+ /\
+ (mitl_general_sem state_holds omega i (mitl_since dm1 iv dm2) =
+  { tau | tau IN omega /\
+   ?j. (SND (tau j)) IN interval_neg_shift (SND (tau i)) iv /\
+    tau IN mitl_general_sem state_holds omega j dm2 /\ 
+     !k. (SND (tau k)) IN { r | (SND (tau j)) <= r /\ r <= (SND (tau i)) } ==>
+      tau IN mitl_general_sem state_holds omega k dm1 })
+ /\
+ (mitl_general_sem state_holds omega i (mitl_box iv dm) = 
+  { tau | tau IN omega /\
+    !j. (SND (tau j)) IN interval_pos_shift (SND (tau i)) iv ==>
+     tau IN mitl_general_sem state_holds omega j dm })
+ /\
+ (mitl_general_sem state_holds omega i (mitl_diamond iv dm) =
+  { tau | tau IN omega /\
+     ?j. (SND (tau j)) IN interval_pos_shift (SND (tau i)) iv /\
+      tau IN mitl_general_sem state_holds omega j dm })
+ /\
+ (mitl_general_sem state_holds omega i (mitl_box_dash iv dm) = 
+  { tau | tau IN omega /\
+    !j. (SND (tau j)) IN interval_neg_shift (SND (tau i)) iv ==>
+     tau IN mitl_general_sem state_holds omega j dm })
+ /\
+ (mitl_general_sem state_holds omega i (mitl_diamond_dash iv dm) = 
+  { tau | tau IN omega /\
+     ?j. (SND (tau j)) IN interval_neg_shift (SND (tau i)) iv /\
+      tau IN mitl_general_sem state_holds omega j dm })
+End
+
+Theorem interval_sem_geq_zero:
+ !iv r. r IN interval_sem iv ==> r >= 0
+Proof
+ Cases_on `iv` >| [
+  rw [interval_sem] >>
+  `0 <= &n` by rw [REAL_POS] >>
+  `0 <= r` suffices_by REAL_ARITH_TAC >>
+  METIS_TAC [REAL_LE_TRANS],
+
+  rw [interval_sem] >>
+  `0 <= &n` by rw [REAL_POS] >>
+  `0 < r` suffices_by REAL_ARITH_TAC >>
+  METIS_TAC [REAL_LET_TRANS],
+
+  rw [interval_sem] >>
+  `0 <= &n` by rw [REAL_POS] >>
+  `0 <= r` suffices_by REAL_ARITH_TAC >>
+  METIS_TAC [REAL_LE_TRANS],
+
+  rw [interval_sem] >>
+  `0 <= &n` by rw [REAL_POS] >>
+  `0 <= r` suffices_by REAL_ARITH_TAC >>
+  METIS_TAC [REAL_LE_TRANS],
+
+  rw [interval_sem] >>
+  `0 <= &n` by rw [REAL_POS] >>
+  `0 < r` suffices_by REAL_ARITH_TAC >>
+  METIS_TAC [REAL_LET_TRANS],
+
+  rw [interval_sem] >>
+  `0 <= &n` by rw [REAL_POS] >>
+  `0 < r` suffices_by REAL_ARITH_TAC >>
+  METIS_TAC [REAL_LET_TRANS]
+ ]
+QED
+
+Theorem timed_word_suffix_eq:
+ !tau. timed_word_suffix tau 0 = tau
+Proof
+ rw [timed_word_suffix,EQ_EXT]
+QED
+
+Theorem timed_word_suffix_suffix:
+ !tau i j.
+  timed_word_suffix (timed_word_suffix tau i) j =
+  timed_word_suffix tau (i + j)
+Proof
+ rw [timed_word_suffix]
+QED
+
+Theorem timed_word_suffix_all_omega:
+ (!i. timed_word_suffix tau i IN omega) ==>
+ tau IN omega
+Proof
+ rw [] >>
+ METIS_TAC [timed_word_suffix_eq]
+QED
+
+Theorem mitl_general_holds_sem:
+ !dm state_holds omega tau k. 
+  (!i. timed_word_suffix tau i IN omega) ==>
+  (mitl_general_holds state_holds tau k dm <=>
+   tau IN mitl_general_sem state_holds omega k dm)
+Proof
+ Induct >> rw [mitl_general_holds,mitl_general_sem] >| [
+  METIS_TAC [timed_word_suffix_eq],
+
+  METIS_TAC [timed_word_suffix_eq],
+
+  METIS_TAC [],
+  
+  EQ_TAC >> rw [] >| [
+   Cases_on `mitl_general_holds state_holds tau k dm'` >-
+   METIS_TAC [] >>
+   `tau IN omega` by rw [timed_word_suffix_all_omega] >>
+   Cases_on `mitl_general_holds state_holds tau k dm` >>
+   METIS_TAC [],
+
+   METIS_TAC [],
+
+   METIS_TAC []
+  ],
+
+  EQ_TAC >> rw [] >| [
+   METIS_TAC [timed_word_suffix_eq],
+   
+   Q.EXISTS_TAC `j` >>
+   METIS_TAC [],
+
+   Q.EXISTS_TAC `j` >>
+   METIS_TAC []   
+  ],
+
+  EQ_TAC >> rw [] >| [
+   METIS_TAC [timed_word_suffix_eq],
+   
+   Q.EXISTS_TAC `j` >>
+   METIS_TAC [],
+
+   Q.EXISTS_TAC `j` >>
+   METIS_TAC []   
+  ],
+
+  EQ_TAC >> rw [] >| [
+   METIS_TAC [timed_word_suffix_eq],
+
+   METIS_TAC [],
+
+   METIS_TAC []
+  ],
+
+  EQ_TAC >> rw [] >| [
+   METIS_TAC [timed_word_suffix_eq],
+   
+   Q.EXISTS_TAC `j` >>
+   METIS_TAC [],
+
+   Q.EXISTS_TAC `j` >>
+   METIS_TAC []   
+  ],
+
+  EQ_TAC >> rw [] >| [
+   METIS_TAC [timed_word_suffix_eq],
+
+   METIS_TAC [],
+
+   METIS_TAC []
+  ],
+
+  EQ_TAC >> rw [] >| [
+   METIS_TAC [timed_word_suffix_eq],
+   
+   Q.EXISTS_TAC `j` >>
+   METIS_TAC [],
+
+   Q.EXISTS_TAC `j` >>
+   METIS_TAC []   
+  ]
+ ]
+QED
+
+Theorem mitl_general_sem_omega:
+ !dm state_holds omega tau k.
+ mitl_general_sem state_holds omega k dm SUBSET omega
+Proof
+ Induct >> rw [mitl_general_sem] >| [
+  rw [SUBSET_DEF],
+
+  `mitl_general_sem state_holds omega k dm' SUBSET omega`
+   by METIS_TAC [] >>
+  `(mitl_general_sem state_holds omega k dm INTER
+    mitl_general_sem state_holds omega k dm') SUBSET
+   mitl_general_sem state_holds omega k dm'`
+   by METIS_TAC [INTER_SUBSET] >>
+  METIS_TAC [SUBSET_TRANS],
+
+  rw [SUBSET_DEF],
+
+  rw [SUBSET_DEF],
+
+  rw [SUBSET_DEF],
+
+  rw [SUBSET_DEF],
+
+  rw [SUBSET_DEF],
+
+  rw [SUBSET_DEF]
+ ]
+QED
+
+(* G_[0,inf) (G_[0,3] b -> F_[3,5] d) *)
+Definition mitl_example:
+ mitl_example (b:string) =
+  (mitl_box (interval_right_half_open_inf 0) (mitl_const b))
+End
+
+val _ = export_theory ();
