README.md
@@ -1,12 +1,12 @@
 # Contract Compositionality
 
-A HOL4 formalization of a theory of specifications, components, contracts, and compositionality. The formalization largely follows a [paper](https://doi.org/10.1007/978-3-030-61467-6_22) by Nyberg, Westman, and Gurov. Some parts build on an [earlier formalization](https://github.com/hedengran/compositionality) by Hedengran.
+A HOL4 formalization of a theory of specifications, components, contracts, and compositionality.
 
 ## Building
 
 Requirements:
-- [Poly/ML 5.8.1](https://github.com/polyml/polyml/releases/tag/v5.8.1) (or later)
-- [HOL4 kananaskis-14](https://github.com/HOL-Theorem-Prover/HOL/releases/tag/kananaskis-14)
+- [Poly/ML 5.7.1](https://github.com/polyml/polyml) (or later)
+- [HOL4 trindemossen-1](https://github.com/HOL-Theorem-Prover/HOL/releases/tag/trindemossen-1)
 
 The default Makefile task, which assumes `Holmake` is available on the system, builds all core HOL4 theories:
 
@@ -19,6 +19,10 @@ make
 - [`folStringScript.sml`](fol/folStringScript.sml): first-order logic with string identifiers
 - [`folStringInterpScript.sml`](fol/folStringInterpScript.sml): some simple first-order theories using string identifiers
 - [`compSpecUtilityScript.sml`](semantics/compSpecUtilityScript.sml): some utility definitions and results
-- [`compSpecScript.sml`](semantics/compSpecScript.sml): definition of abstract syntax for specifications, components, and predicates, and definition of proof system
+- [`compSpecScript.sml`](semantics/compSpecScript.sml): definition of abstract syntax for specifications, components, and predicates, and definition of proof systems
 - [`compSpecMetaScript.sml`](semantics/compSpecMetaScript.sml): semantics and metatheory of specifications and components, including proof system soundness
 - [`compSpecFolScript.sml`](semantics/compSpecFolScript.sml): interpretation as first-order theory
+- [`compSpecFolScript.sml`](semantics/compSpecFolScript.sml): interpretation as first-order theory
+- [`mitlScript.sml`](semantics/mitlScript.sml): MITL formal semantics
+- [`compSpecMitlScript.sml`](semantics/compSpecMitlScript.sml): instantiation of specifications for MITL
+- [`compSpecMitlFLDScript.sml`](semantics/compSpecMitlFLDScript.sml): instantiation for a fuel level display (FLD) system
